theories/rust_typing/value.v
@@ -77,10 +77,34 @@ Section value.
         try match type of Hot with | _ ∧ _  => destruct Hot end; subst; done.
   Qed.
 
-  Global Instance value_t_copy st : Copyable (value_t st).
+  Global Instance value_copy st : Copyable (value_t st).
   Proof. apply _. Qed.
+End value.
 
-  Lemma value_split π {rt} (ty : type rt) r v st ly :
+Section lemmas.
+  Context `{!typeGS Σ}.
+
+  Lemma value_has_length π v v1 st ly :
+    syn_type_has_layout st ly →
+    v ◁ᵥ{π} v1 @ value_t st -∗
+    ⌜length v1 = ly_size ly⌝ ∗ ⌜length v = ly_size ly⌝.
+  Proof.
+    rewrite /ty_own_val/=.
+    iDestruct 1 as "(%ot & %Hot & %Hmc & %Hly & %Hst)".
+    assert (ly = ot_layout ot) as -> by by eapply syn_type_has_layout_inj.
+    iL. iPureIntro. apply is_memcast_val_length in Hmc as ->; done.
+  Qed.
+
+  Lemma value_has_layout π st v vs :
+    v ◁ᵥ{π} vs @ value_t st -∗
+    ∃ ly, ⌜syn_type_has_layout st ly⌝ ∗ ⌜v `has_layout_val` ly⌝.
+  Proof.
+    rewrite /ty_own_val.
+    iDestruct 1 as "(%ot & %Hot & %Hmv & %Hv & %Hst)".
+    iExists (ot_layout ot). iR. done.
+  Qed.
+
+  Lemma own_val_split_value π {rt} (ty : type rt) r v st ly :
     syn_type_has_layout (ty_syn_type ty) ly ∧ syn_type_has_layout st ly →
     v ◁ᵥ{π} r @ ty -∗
     v ◁ᵥ{π} v @ value_t st ∗ v ◁ᵥ{π} r @ ty.
@@ -94,8 +118,8 @@ Section value.
     done.
   Qed.
 
-  Lemma value_make_typed π st ly v vs :
-    ⌜syn_type_has_layout st ly⌝ -∗
+  Lemma value_untyped_make_typed π st ly v vs :
+    syn_type_has_layout st ly →
     v ◁ᵥ{π} vs @ value_t (UntypedSynType ly) -∗
     v ◁ᵥ{π} vs @ value_t st.
   Proof.
@@ -108,23 +132,7 @@ Section value.
     iSplitR; first done. done.
   Qed.
 
-  (* TODO move *)
-  Lemma ly_size_ly_offset ly n :
-    ly_size (ly_offset ly n) = ly_size ly - n.
-  Proof.
-    rewrite /ly_size /ly_offset. destruct ly; done.
-  Qed.
-  Lemma layout_wf_mono ly1 ly2 :
-    ly_align_log ly2 ≤ ly_align_log ly1 →
-    ly_size ly1 = ly_size ly2 →
-    layout_wf ly1 → layout_wf ly2.
-  Proof.
-    rewrite /layout_wf /ly_align. intros Hle Hsz Hdiv.
-    rewrite -Hsz. eapply Z.divide_trans; last apply Hdiv.
-    eapply Zdivide_nat_pow. done.
-  Qed.
-
-  Lemma value_untyped_mono π v vs ly1 ly2 :
+  Lemma value_untyped_layout_mono π v vs ly1 ly2 :
     ly_size ly1 = ly_size ly2 →
     (layout_wf ly1 → layout_wf ly2) →
     (ly_align_in_bounds ly1 → ly_align_in_bounds ly2) →
@@ -144,89 +152,7 @@ Section value.
     - by apply Hal.
   Qed.
 
-  (* TODO move *)
-  Lemma ofty_mono_ly_strong_in π {rt1 rt2} l wl (ty1 : type rt1) (ty2 : type rt2) (r1 : rt1) (r2 : rt2) ly1 ly2 :
-    syn_type_has_layout (ty1.(ty_syn_type)) ly1 →
-    syn_type_has_layout (ty2.(ty_syn_type)) ly2 →
-    (l `has_layout_loc` ly1 → l `has_layout_loc` ly2) →
-    ly_size ly2 = ly_size ly1 →
-    (∀ v, ty1.(ty_own_val) π r1 v -∗ ty2.(ty_own_val) π r2 v) -∗
-    (ty_sidecond ty1 -∗ ty_sidecond ty2) -∗
-    l ◁ₗ[π, Owned wl] #r1 @ (◁ ty1) -∗
-    l ◁ₗ[π, Owned wl] #r2 @ (◁ ty2).
-  Proof.
-    intros Halg1 Halg2 Halign Hsz. iIntros "Hvs Hscvs Hl".
-    rewrite !ltype_own_ofty_unfold /lty_of_ty_own.
-    iDestruct "Hl" as "(%ly1' & %Halg1' & %Hly & Hsc & Hlb & Hcred & %r' & <- & Hb)".
-    assert (ly1' = ly1) as -> by by eapply syn_type_has_layout_inj.
-    iExists ly2. iSplitR; first done.
-    iSplitR. { iPureIntro. by apply Halign. }
-    iPoseProof ("Hscvs" with "Hsc") as "$".
-    rewrite Hsz. iFrame "Hlb Hcred".
-    iExists r2. iSplitR; first done.
-    iNext. iMod "Hb" as "(%v & Hl & Hv)".
-    iModIntro. iExists v. iFrame. by iApply "Hvs".
-  Qed.
-  Lemma ofty_mono_ly_strong π {rt1} l wl (ty1 : type rt1) (ty2 : type rt1) (r1 : place_rfn rt1) ly1 ly2 :
-    syn_type_has_layout (ty1.(ty_syn_type)) ly1 →
-    syn_type_has_layout (ty2.(ty_syn_type)) ly2 →
-    (l `has_layout_loc` ly1 → l `has_layout_loc` ly2) →
-    ly_size ly2 = ly_size ly1 →
-    (∀ v r, ty1.(ty_own_val) π r v -∗ ty2.(ty_own_val) π r v) -∗
-    (ty_sidecond ty1 -∗ ty_sidecond ty2) -∗
-    l ◁ₗ[π, Owned wl] r1 @ (◁ ty1) -∗
-    l ◁ₗ[π, Owned wl] r1 @ (◁ ty2).
-  Proof.
-    intros Halg1 Halg2 Halign Hsz. iIntros "Hvs Hscvs Hl".
-    rewrite !ltype_own_ofty_unfold /lty_of_ty_own.
-    iDestruct "Hl" as "(%ly1' & %Halg1' & %Hly & Hsc & Hlb & Hcred & %r' & ? & Hb)".
-    assert (ly1' = ly1) as -> by by eapply syn_type_has_layout_inj.
-    iExists ly2. iSplitR; first done.
-    iSplitR. { iPureIntro. by apply Halign. }
-    iPoseProof ("Hscvs" with "Hsc") as "$".
-    rewrite Hsz. iFrame "Hlb Hcred".
-    iExists _. iFrame.
-    iNext. iMod "Hb" as "(%v & Hl & Hv)".
-    iModIntro. iExists v. iFrame. by iApply "Hvs".
-  Qed.
-
-  Lemma value_split_ofty_untyped π F l {rt} (ty : type rt) r ly :
-    lftE ⊆ F →
-    syn_type_has_layout (ty_syn_type ty) ly →
-    (l ◁ₗ[π, Owned false] #r @ ◁ ty)%I ={F}=∗ ∃ v,
-    v ◁ᵥ{π} r @ ty ∗ l ◁ₗ[π, Owned false] #v @ ◁ (value_t (UntypedSynType ly)).
-  Proof.
-    iIntros (? Halg) "Hty".
-    rewrite (ltype_own_ofty_unfold ty) /lty_of_ty_own.
-    iDestruct "Hty" as "(%ly' & % & % & Hsc & Hlb & _ & %r' & <- & Hb)".
-    assert (ly' = ly) as -> by by eapply syn_type_has_layout_inj.
-    iMod (fupd_mask_mono with "Hb") as "(%v & Hl & Hv)"; first done.
-    iPoseProof (value_split _ _ _ _ (UntypedSynType _) with "Hv") as "(Hv' & Hv)".
-    { split; first done. eapply syn_type_has_layout_make_untyped; done. }
-    iExists v. iFrame.
-    rewrite ltype_own_ofty_unfold /lty_of_ty_own.
-    iExists _. simpl.
-    iSplitR. { iPureIntro. eapply syn_type_has_layout_make_untyped; done. }
-    iSplitR; first done. iFrame. iSplitR; first done.
-    iExists _. iSplitR; first done. iModIntro.
-    iExists v. by iFrame.
-  Qed.
-
-  Lemma mem_cast_UntypedOp v ly st :
-    mem_cast v (UntypedOp ly) st = v.
-  Proof. done. Qed.
-  Lemma is_memcast_val_untyped_app ly1 ly2 ly3 v1 v2 v1' v2' :
-    ly_size ly3 = ly_size ly1 + ly_size ly2 →
-    is_memcast_val v1 (UntypedOp ly1) v1' →
-    is_memcast_val v2 (UntypedOp ly2) v2' →
-    is_memcast_val (v1 ++ v2) (UntypedOp ly3) (v1' ++ v2').
-  Proof.
-    intros Hsz H1 H2.
-    destruct H1 as [->  | (st1 & ->)]; destruct H2 as [-> | (st2 & ->)]; simpl;
-        try rewrite !mem_cast_UntypedOp; by left.
-  Qed.
-
-  Lemma value_t_app_untyped π v1 v2 r1 r2 ly1 ly2 ly3 :
+  Lemma value_untyped_app_merge π v1 v2 r1 r2 ly1 ly2 ly3 :
     syn_type_has_layout (UntypedSynType ly3) ly3 →
     ly_size ly3 = ly_size ly1 + ly_size ly2 →
     v1 ◁ᵥ{π} r1 @ value_t (UntypedSynType ly1) -∗
@@ -249,37 +175,147 @@ Section value.
     - done.
   Qed.
 
-  Lemma ofty_uninit_to_value_t F π l st :
+  Lemma value_untyped_app_split π v v1 v2 ly1 ly2 ly3 :
+    ly_size ly1 = ly_size ly2 + ly_size ly3 →
+    length v1 = ly_size ly2 →
+    layout_wf ly2 →
+    layout_wf ly3 →
+    ly_align_in_bounds ly3 →
+    ly_align_in_bounds ly2 →
+    v ◁ᵥ{π} (v1 ++ v2) @ value_t (UntypedSynType ly1) -∗
+    (take (length v1) v) ◁ᵥ{π} v1 @ value_t (UntypedSynType ly2) ∗
+    (drop (length v1) v) ◁ᵥ{π} v2 @ value_t (UntypedSynType ly3).
+  Proof.
+    iIntros (Hsz ?????) "Hv".
+    rewrite /ty_own_val/=. iDestruct "Hv" as "(%ot & %Hot & %Hmc & %Hly & %Hst)".
+    apply use_op_alg_untyped_inv in Hot as ->.
+    apply syn_type_has_layout_untyped_inv in Hst as (<- & Hwf & Hsz' & ?).
+    apply is_memcast_val_untyped_inv in Hmc as <-.
+    rewrite /has_layout_val/= app_length in Hly.
+    simpl in *.
+    iSplit.
+    - iPureIntro. exists (UntypedOp ly2). split; first done.
+      split. { left. rewrite take_app//. }
+      split. { rewrite take_app. rewrite /has_layout_val/=. lia. }
+      apply syn_type_has_layout_untyped; try naive_solver lia.
+    - iPureIntro. exists (UntypedOp ly3). split; first done.
+      split. { left. rewrite drop_app//. }
+      split. { rewrite drop_app. rewrite /has_layout_val/=. lia. }
+      apply syn_type_has_layout_untyped; naive_solver lia.
+  Qed.
+End lemmas.
+
+Section ofty_lemmas.
+  Context `{!typeGS Σ}.
+
+  Lemma ofty_value_has_length F π l st ly v1 :
+    lftE ⊆ F →
+    syn_type_has_layout st ly →
+    l ◁ₗ[π, Owned false] #v1 @ (◁ value_t st) ={F}=∗
+    ⌜length v1 = ly_size ly⌝ ∗ l ◁ₗ[π, Owned false] #v1 @ (◁ value_t st).
+  Proof.
+    iIntros (??) "Hl".
+    rewrite ltype_own_ofty_unfold/lty_of_ty_own.
+    iDestruct "Hl" as "(%ly' & % & % & ? & ? & ? & %r' & <- & Hb)".
+    iMod (fupd_mask_mono with "Hb") as "(%v & Hl & Hv)"; first done.
+    iPoseProof (value_has_length with "Hv") as "(% & %)"; first done.
+    assert (ly' = ly) as -> by by eapply syn_type_has_layout_inj.
+    iR. iModIntro. iExists _. iFrame. iR. iR. iExists _. iR.
+    iModIntro. eauto with iFrame.
+  Qed.
+
+  (* NOTE: We can make this into a typed value afterwards using [ofty_value_untyped_make_typed] *)
+  Lemma ofty_own_split_value_untyped π F l {rt} (ty : type rt) r ly :
+    lftE ⊆ F →
+    syn_type_has_layout (ty_syn_type ty) ly →
+    (l ◁ₗ[π, Owned false] #r @ ◁ ty)%I ={F}=∗ ∃ v,
+    v ◁ᵥ{π} r @ ty ∗ l ◁ₗ[π, Owned false] #v @ ◁ (value_t (UntypedSynType ly)).
+  Proof.
+    iIntros (? Halg) "Hty".
+    rewrite (ltype_own_ofty_unfold ty) /lty_of_ty_own.
+    iDestruct "Hty" as "(%ly' & % & % & Hsc & Hlb & _ & %r' & <- & Hb)".
+    assert (ly' = ly) as -> by by eapply syn_type_has_layout_inj.
+    iMod (fupd_mask_mono with "Hb") as "(%v & Hl & Hv)"; first done.
+    iPoseProof (own_val_split_value _ _ _ _ (UntypedSynType _) with "Hv") as "(Hv' & Hv)".
+    { split; first done. eapply syn_type_has_layout_make_untyped; done. }
+    iExists v. iFrame.
+    rewrite ltype_own_ofty_unfold /lty_of_ty_own.
+    iExists _. simpl.
+    iSplitR. { iPureIntro. eapply syn_type_has_layout_make_untyped; done. }
+    iSplitR; first done. iFrame. iSplitR; first done.
+    iExists _. iSplitR; first done. iModIntro.
+    iExists v. by iFrame.
+  Qed.
+
+  (* TODO ideally, the requirement for the UntypedOp case should just generally hold for types. Untyped should always be possible. *)
+  Lemma ofty_own_merge_value {rt} π (ty : type rt) wl v r st l :
+    match st with
+    | UntypedSynType ly1 =>
+        syn_type_has_layout (ty_syn_type ty) ly1 ∧ ty_has_op_type ty (UntypedOp ly1) MCCopy
+    | _ =>
+        ty_has_op_type ty (use_op_alg' (ty_syn_type ty)) MCCopy ∧ ty_syn_type ty = st
+    end →
+    v ◁ᵥ{ π} r @ ty -∗
+    l ◁ₗ[ π, Owned wl] #v @ (◁ value_t st) -∗
+    l ◁ₗ[ π, Owned wl] #r @ (◁ ty).
+  Proof.
+    iIntros (?) "Hv Hl".
+    rewrite !ltype_own_ofty_unfold /lty_of_ty_own.
+    iDestruct "Hl" as "(%ly & %Halg & % & Hsc & Hlb & Hcred & %r' & Hrfn & Hb)".
+    simpl in Halg.
+    iExists ly.
+    iFrame. iFrame "%".
+    iPoseProof (ty_own_val_sidecond with "Hv") as "#$".
+    assert ((∃ ly1, st = UntypedSynType ly1 ∧ syn_type_has_layout (ty_syn_type ty) ly1 ∧ ty_has_op_type ty (UntypedOp ly1) MCCopy) ∨ (ty_has_op_type ty (use_op_alg' (ty_syn_type ty)) MCCopy ∧ ty_syn_type ty = st)) as Hb.
+    { destruct st; eauto. }
+    iSplitR. { iPureIntro. destruct Hb as [(ly1 & -> & ? & ?) | (? & <-)]; last done.
+      apply syn_type_has_layout_untyped_inv in Halg as (-> & _). done. }
+    iExists r. iSplitR; first done.
+    iNext. iMod "Hb" as "(%v' & Hl & Hv')". iModIntro.
+    iDestruct "Hrfn" as "<-".
+    iExists v'. iFrame.
+    iEval (rewrite /ty_own_val/=) in "Hv'".
+    iDestruct "Hv'" as "(%ot & %Hot' & %Hmc & %Hv & ?)".
+    destruct Hmc as [-> | [st' ->]]; first done.
+    iApply (ty_memcast_compat_copy with "Hv").
+
+    destruct Hb as [(ly1 & -> & Hst & ?) | (Hst & <-)].
+    - injection Hot' as <-. done.
+    - move: Hst. rewrite /use_op_alg' Hot' //.
+  Qed.
+
+  Lemma ofty_value_untyped_make_typed π l vs st ly wl :
+    syn_type_has_layout st ly →
+    (l ◁ₗ[π, Owned wl] #vs @ ◁ value_t (UntypedSynType ly)) -∗
+    l ◁ₗ[π, Owned wl] #vs @ ◁ value_t st.
+  Proof.
+    iIntros (?) "Ha".
+    iApply (ofty_mono_ly_strong_in with "[] [] Ha").
+    - simpl. by eapply syn_type_has_layout_make_untyped.
+    - done.
+    - done.
+    - done.
+    - iIntros (?). by iApply value_untyped_make_typed.
+    - simpl. eauto.
+  Qed.
+
+  Lemma ofty_uninit_to_value F π l st :
     lftE ⊆ F →
     (l ◁ₗ[π, Owned false] .@ ◁ (uninit st))%I ={F}=∗
     ∃ v, l ◁ₗ[π, Owned false] #v @ (◁ value_t st)%I.
   Proof.
-    iIntros (?) "Hl".
-    rewrite ltype_own_ofty_unfold /lty_of_ty_own.
-    iDestruct "Hl" as "(%ly & %Halg & %Hly & _ & Hlb & _ & %r' & <- & Hb)".
-    iMod (fupd_mask_mono with "Hb") as "Hb"; first done.
-    iDestruct "Hb" as "(%v & Hl & Hv)".
-    iExists v. rewrite ltype_own_ofty_unfold /lty_of_ty_own.
-    iExists ly. iR. iR. iR. iFrame. iR. iExists v. iR.
-    iModIntro. iNext. iModIntro. iExists v. iFrame.
-    rewrite /ty_own_val/=.
-    destruct (syn_type_has_layout_op_alg _ _ Halg) as (ot & Hot & Hly').
-    iExists ot.
-    iR.
-    iDestruct "Hv" as "(%ly'' & %Halg' & %Hlyv & _)".
-    assert (ly'' = ly) as -> by by eapply syn_type_has_layout_inj.
-    iSplitR. { iPureIntro. left. done. }
-    iSplitR. { iPureIntro. rewrite /has_layout_val Hly'//. }
-    iPureIntro. rewrite Hly'. done.
+    iIntros (?) "Ha".
+    iPoseProof (ltype_own_has_layout with "Ha") as "(%ly & %Hst & %Hly)".
+    simp_ltypes in Hst. simpl in Hst.
+    iMod (ofty_own_split_value_untyped with "Ha") as "(%v & _ & Ha)"; [done.. | ].
+    iExists v. by iApply (ofty_value_untyped_make_typed with "Ha").
   Qed.
 
-
-  Lemma ofty_value_t_untyped_reduce_alignment π l vs ly1 ly2 :
+  Lemma ofty_value_untyped_reduce_alignment π l vs ly1 ly2 :
     ly_size ly1 = ly_size ly2 →
     l `has_layout_loc` ly2 →
     layout_wf ly2 →
     (ly_align_in_bounds ly1 → ly_align_in_bounds ly2) →
-    (*ly_align_log ly2 ≤ ly_align_log ly1 →*)
     (l ◁ₗ[π, Owned false] vs @ ◁ value_t (UntypedSynType ly1)) -∗
     (l ◁ₗ[π, Owned false] vs @ ◁ value_t (UntypedSynType ly2)).
   Proof.
@@ -295,10 +331,11 @@ Section value.
       - by apply Halmon.
     + done.
     + done.
-    + iIntros (??). iApply value_untyped_mono; [done.. | ]. eauto.
+    + iIntros (??). iApply value_untyped_layout_mono; [done.. | ]. eauto.
     + simpl. done.
   Qed.
-  Lemma ofty_value_t_merge_adjacent π l vs1 vs2 ly1 ly2 ly3 :
+
+  Lemma ofty_value_untyped_app_merge π l vs1 vs2 ly1 ly2 ly3 :
     l `has_layout_loc` ly3 →
     ly_size ly1 ≤ ly_size ly3 →
     ly_size ly2 = ly_size ly3 - ly_size ly1 →
@@ -329,65 +366,14 @@ Section value.
     iPoseProof (ty_has_layout with "Hv1") as "(%ly' & %Halg & %Hlyv)".
     apply syn_type_has_layout_untyped_inv in Halg as (-> & ? & ?).
     iSplitL "Hl2". { rewrite /has_layout_val in Hlyv. rewrite Hlyv. done. }
-    iApply (value_t_app_untyped with "Hv1 Hv2").
+    iApply (value_untyped_app_merge with "Hv1 Hv2").
     - done.
     - rewrite Hlysz. lia.
   Qed.
 
-  (* TODO move *)
-  Lemma use_op_alg_untyped_inv ly ot :
-    use_op_alg (UntypedSynType ly) = Some ot → ot = (UntypedOp ly).
-  Proof.
-    rewrite /use_op_alg.
-    intros [= <-]; done.
-  Qed.
-
-  Lemma value_t_app_split_untyped π v v1 v2 ly1 ly2 ly3 :
-    ly_size ly1 = ly_size ly2 + ly_size ly3 →
-    length v1 = ly_size ly2 →
-    layout_wf ly2 →
-    layout_wf ly3 →
-    ly_align_in_bounds ly3 →
-    ly_align_in_bounds ly2 →
-    v ◁ᵥ{π} (v1 ++ v2) @ value_t (UntypedSynType ly1) -∗
-    (take (length v1) v) ◁ᵥ{π} v1 @ value_t (UntypedSynType ly2) ∗
-    (drop (length v1) v) ◁ᵥ{π} v2 @ value_t (UntypedSynType ly3).
-  Proof.
-    iIntros (Hsz ?????) "Hv".
-    rewrite /ty_own_val/=. iDestruct "Hv" as "(%ot & %Hot & %Hmc & %Hly & %Hst)".
-    apply use_op_alg_untyped_inv in Hot as ->.
-    apply syn_type_has_layout_untyped_inv in Hst as (<- & Hwf & Hsz' & ?).
-    apply is_memcast_val_untyped_inv in Hmc as <-.
-    rewrite /has_layout_val/= app_length in Hly.
-    simpl in *.
-    iSplit.
-    - iPureIntro. exists (UntypedOp ly2). split; first done.
-      split. { left. rewrite take_app//. }
-      split. { rewrite take_app. rewrite /has_layout_val/=. lia. }
-      apply syn_type_has_layout_untyped; try naive_solver lia.
-    - iPureIntro. exists (UntypedOp ly3). split; first done.
-      split. { left. rewrite drop_app//. }
-      split. { rewrite drop_app. rewrite /has_layout_val/=. lia. }
-      apply syn_type_has_layout_untyped; naive_solver lia.
-  Qed.
-
-  (* TODO move *)
-  Lemma ly_align_in_bounds_mono ly1 ly2 :
-    ly_align_log ly2 ≤ ly_align_log ly1 →
-    ly_align_in_bounds ly1 →
-    ly_align_in_bounds ly2.
-  Proof.
-    rewrite /ly_align_in_bounds.
-    intros Hle. rewrite /ly_align/min_alloc_start. intros Ha.
-    split.
-    - specialize (Nat_pow_ge_1 (ly_align_log ly2)). lia.
-    - etrans; last apply Ha.
-      apply inj_le. apply Nat.pow_le_mono_r; done.
-  Qed.
-
-  Lemma ofty_value_t_split_adjacent F π l v1 v2 v3 ly1 ly2 ly3 :
+  Lemma ofty_value_untyped_app_split F π l v1 v2 v3 ly1 ly2 ly3 :
     lftE ⊆ F →
-    ly_align_log ly3 ≤ ly_align_log ly1 →
+    ly_align_log ly3 ≤ ly_align_log ly2 →
     ly_align_log ly2 ≤ ly_align_log ly1 →
     ly_size ly1 = ly_size ly2 + ly_size ly3 →
     v1 = v2 ++ v3 →
@@ -398,15 +384,17 @@ Section value.
     l ◁ₗ[π, Owned false] #v2 @ (◁ value_t (UntypedSynType ly2)) ∗
     (l +ₗ ly_size ly2) ◁ₗ[π, Owned false] #v3 @ ◁ value_t (UntypedSynType ly3).
   Proof.
-    iIntros (? Hal3 Hal2 Hsz -> Hszeq ??) "Hl".
+    iIntros (? Hal3 Hal2 Hsz -> Hszeq Hwf2 Hwf3) "Hl".
     rewrite ltype_own_ofty_unfold /lty_of_ty_own.
     iDestruct "Hl" as "(%ly & %Halg & %Hly & Hsc & Hlb & _ & %r' & <- & Hb)".
     iMod (fupd_mask_mono with "Hb") as "(%v & Hl & Hv)"; first done.
-    apply syn_type_has_layout_untyped_inv in Halg as (-> & ? & ? &?).
+    specialize (syn_type_has_layout_untyped_inv _ _  Halg) as (-> & ? & ? &?).
     rewrite Hsz. rewrite -loc_in_bounds_split_suf. iDestruct "Hlb" as "(Hlb1 & Hlb2)".
     efeed pose proof (ly_align_in_bounds_mono ly1 ly2); [done.. | ].
-    efeed pose proof (ly_align_in_bounds_mono ly1 ly3); [done.. | ].
-    iPoseProof (value_t_app_split_untyped _ _ _ _ ly1 ly2 ly3 with "Hv") as "(Hv1 & Hv2)".
+    efeed pose proof (ly_align_in_bounds_mono ly1 ly3); [lia | done | ].
+    iPoseProof (value_has_length with "Hv") as "(%Hlen1 & %Hlen2)"; first done.
+    rewrite app_length in Hlen1.
+    iPoseProof (value_untyped_app_split _ _ _ _ ly1 ly2 ly3 with "Hv") as "(Hv1 & Hv2)".
     { done. }
     { done. }
     { done. }
@@ -423,57 +411,17 @@ Section value.
       iModIntro. iExists _. iFrame.
     - iModIntro. rewrite ltype_own_ofty_unfold /lty_of_ty_own.
       iExists ly3. iSplitR. { iPureIntro. apply syn_type_has_layout_untyped; naive_solver lia. }
-      iSplitR. { iPureIntro. admit. }
+      iSplitR. { iPureIntro. apply has_layout_loc_shift_loc_nat.
+        + eapply has_layout_loc_trans; first done. lia.
+        + trans (ly_align ly2); first last. { rewrite -Nat2Z.divide//. }
+          rewrite -Nat2Z.divide. apply Zdivide_nat_pow. done. }
       simpl. iR. iFrame. iExists v3. iR.
       iModIntro. iExists _. iFrame.
       rewrite take_length. rewrite Hszeq Nat.min_l; first done.
-      (* length v1 = ly_size ly1  *)
-  Admitted.
-
-  Lemma ofty_value_t_untyped_to_bytes π l vn ly :
-    l ◁ₗ[π, Owned false] #vn @ (◁ value_t (UntypedSynType ly)) -∗
-    l ◁ₗ[π, Owned false] #vn @ (◁ value_t (UntypedSynType $ mk_array_layout u8 (ly_size ly))).
-  Proof.
-    (* We can always go to something with a lower alignment *)
-    iIntros "Hl". iPoseProof (ltype_own_has_layout with "Hl") as "(%ly' & %Halg & %Hly)".
-    simp_ltypes in Halg. simpl in Halg.
-    apply syn_type_has_layout_untyped_inv in Halg as (-> & ? & ?).
-    iApply (ofty_value_t_untyped_reduce_alignment with "Hl").
-    - rewrite /mk_array_layout/u8{2}/ly_size/=. lia.
-    - rewrite /has_layout_loc/ly_align/mk_array_layout/u8/=.
-      rewrite /aligned_to. destruct caesium_config.enforce_alignment; last done.
-      apply Z.divide_1_l.
-    - rewrite /layout_wf/ly_align/u8/=. apply Z.divide_1_l.
-    - done.
+      lia.
   Qed.
 
-  Lemma value_t_has_length π v v1 st ly :
-    syn_type_has_layout st ly →
-    v ◁ᵥ{π} v1 @ value_t st -∗
-    ⌜length v1 = ly_size ly⌝ ∗ ⌜length v = ly_size ly⌝.
-  Proof.
-    rewrite /ty_own_val/=.
-    iDestruct 1 as "(%ot & %Hot & %Hmc & %Hly & %Hst)".
-    assert (ly = ot_layout ot) as -> by by eapply syn_type_has_layout_inj.
-    iL. iPureIntro. apply is_memcast_val_length in Hmc as ->; done.
-  Qed.
-  Lemma ofty_value_t_has_length F π l st ly v1 :
-    lftE ⊆ F →
-    syn_type_has_layout st ly →
-    l ◁ₗ[π, Owned false] #v1 @ (◁ value_t st) ={F}=∗
-    ⌜length v1 = ly_size ly⌝ ∗ l ◁ₗ[π, Owned false] #v1 @ (◁ value_t st).
-  Proof.
-    iIntros (??) "Hl".
-    rewrite ltype_own_ofty_unfold/lty_of_ty_own.
-    iDestruct "Hl" as "(%ly' & % & % & ? & ? & ? & %r' & <- & Hb)".
-    iMod (fupd_mask_mono with "Hb") as "(%v & Hl & Hv)"; first done.
-    iPoseProof (value_t_has_length with "Hv") as "(% & %)"; first done.
-    assert (ly' = ly) as -> by by eapply syn_type_has_layout_inj.
-    iR. iModIntro. iExists _. iFrame. iR. iR. iExists _. iR.
-    iModIntro. eauto with iFrame.
-  Qed.
-
-  Lemma ofty_value_t_untyped_split_adjacent_array F π l (n m k : nat) ly v1 :
+  Lemma ofty_value_untyped_split_app_array F π l (n m k : nat) ly v1 :
     lftE ⊆ F →
     n = (m + k)%nat →
     layout_wf ly →
@@ -487,9 +435,9 @@ Section value.
     iIntros "Hl".
     iPoseProof (ltype_own_has_layout with "Hl") as "(%lyv & %Hstly & %Hlyl)".
     simp_ltypes in Hstly. simpl in Hstly.
-    iMod (ofty_value_t_has_length with "Hl") as "(%Hlen & Hl)"; [done.. | ].
+    iMod (ofty_value_has_length with "Hl") as "(%Hlen & Hl)"; [done.. | ].
     simpl in *.
-    iApply (ofty_value_t_split_adjacent with "Hl").
+    iApply (ofty_value_untyped_app_split with "Hl").
     - done.
     - simpl. lia.
     - simpl. lia.
@@ -502,15 +450,23 @@ Section value.
     - by apply array_layout_wf.
   Qed.
 
-  Lemma value_t_has_layout π st v vs :
-    v ◁ᵥ{π} vs @ value_t st -∗
-    ∃ ly, ⌜syn_type_has_layout st ly⌝ ∗ ⌜v `has_layout_val` ly⌝.
+  Lemma ofty_value_untyped_to_bytes π l vn ly :
+    l ◁ₗ[π, Owned false] #vn @ (◁ value_t (UntypedSynType ly)) -∗
+    l ◁ₗ[π, Owned false] #vn @ (◁ value_t (UntypedSynType $ mk_array_layout u8 (ly_size ly))).
   Proof.
-    rewrite /ty_own_val.
-    iDestruct 1 as "(%ot & %Hot & %Hmv & %Hv & %Hst)".
-    iExists (ot_layout ot). iR. done.
+    (* We can always go to something with a lower alignment *)
+    iIntros "Hl". iPoseProof (ltype_own_has_layout with "Hl") as "(%ly' & %Halg & %Hly)".
+    simp_ltypes in Halg. simpl in Halg.
+    apply syn_type_has_layout_untyped_inv in Halg as (-> & ? & ?).
+    iApply (ofty_value_untyped_reduce_alignment with "Hl").
+    - rewrite /mk_array_layout/u8{2}/ly_size/=. lia.
+    - rewrite /has_layout_loc/ly_align/mk_array_layout/u8/=.
+      rewrite /aligned_to. destruct caesium_config.enforce_alignment; last done.
+      apply Z.divide_1_l.
+    - rewrite /layout_wf/ly_align/u8/=. apply Z.divide_1_l.
+    - done.
   Qed.
-End value.
+End ofty_lemmas.
 
 Global Hint Unfold value_t : tyunfold.
 Global Typeclasses Opaque value_t.
@@ -518,17 +474,20 @@ Global Typeclasses Opaque value_t.
 (** ** value rules *)
 Section rules.
   Context `{!typeGS Σ}.
+  (** *** Rules converting other types to/from values*)
+  (** NOTE: This needs to have lower priority than the below subsumption instances that specialize to the case where [ty = value_t _].
+     In addition, other rules for other types should similarly be able to implement their own proof strategies.
+     Namely, this rule makes a pretty strong commitment (having an exactly fitting value assignment available),
+     so we should really try it as a last resort. So we give it a pretty low priority. *)
 
-
-  (** *** instances for types that are not value -- these have lower priority than the the value-specific versions below *)
-  (** by default, we go to UntypedSynType, and can later on specialize if needed by subsumption (we cannot go the other way around due to memcast compatibility) *)
+  (** By default, we go to UntypedSynType, and can later on specialize if needed by subsumption (we cannot go the other way around due to memcast compatibility) *)
   Lemma value_subsume_goal π {rt} (ty : type rt) (r : rt) v vs st T :
     (∃ ly, ⌜syn_type_has_layout ty.(ty_syn_type) ly⌝ ∗
       (v ◁ᵥ{π} r @ ty -∗ subsume (v ◁ᵥ{π} v @ value_t (UntypedSynType ly)) (v ◁ᵥ{π} vs @ value_t st) T))
     ⊢ subsume (v ◁ᵥ{π} r @ ty) (v ◁ᵥ{π} vs @ value_t st) T.
   Proof.
     iIntros "(%ly & %Halg & HT) Hv".
-    iPoseProof (value_split _ _ _ _ (UntypedSynType _) with "Hv") as "(Hv' & Hv)".
+    iPoseProof (own_val_split_value _ _ _ _ (UntypedSynType _) with "Hv") as "(Hv' & Hv)".
     { split; first done. eapply syn_type_has_layout_make_untyped; done. }
     iApply ("HT" with "Hv Hv'").
   Qed.
@@ -543,11 +502,12 @@ Section rules.
     li_tactic (compute_layout_goal ty.(ty_syn_type)) (λ ly,
       (∀ v, v ◁ᵥ{π} r @ ty -∗
       subsume_full E L step (l ◁ₗ[π, Owned false] #v @ ◁ value_t (UntypedSynType ly)) (l ◁ₗ[π, Owned false] #v' @ ◁ (value_t st)) T))
-    ⊢ subsume_full E L step (l ◁ₗ[π, Owned false] #r @ ◁ ty) (l ◁ₗ[π, Owned false] #v' @ ◁ (value_t st)) T.
+    ⊢ subsume_full E L step (l ◁ₗ[π, Owned false] #r @ ◁ ty)
+        (l ◁ₗ[π, Owned false] #v' @ ◁ (value_t st)) T.
   Proof.
     rewrite /compute_layout_goal.
     iIntros "(%ly & %Hst & HT)" (???) "#CTX #HE HL Hty".
-    iMod (value_split_ofty_untyped with "Hty") as "(%v & Hv & Hty)"; [done.. | ].
+    iMod (ofty_own_split_value_untyped with "Hty") as "(%v & Hv & Hty)"; [done.. | ].
     iDestruct ("HT" with "Hv") as "HT".
     by iApply ("HT" with "[//] [//] CTX HE HL").
   Qed.
@@ -556,8 +516,72 @@ Section rules.
     (*SubsumeFull E L (l ◁ₗ[π, Owned false] PlaceIn r @ ◁ ty)%I (l ◁ₗ[π, Owned false] PlaceIn v' @ ◁ (value_t st))%I | 50 :=*)
     (*λ T, i2p (value_subsume_full_goal_ofty π E L l v' st ty r T).*)
 
+  (** When we require assembled ownership, try to assemble it. *)
 
+  Lemma subsume_full_value_merge_ofty_untyped {rt} π E L (ty : type rt) r v l ly1 wl T :
+    (prove_with_subtype E L false ProveDirect (v ◁ᵥ{π} r @ ty) (λ L' _ R,
+      ⌜syn_type_has_layout ty.(ty_syn_type) ly1⌝ ∗ ⌜ty_has_op_type ty (UntypedOp ly1) MCCopy⌝ ∗ T L' R))
+    ⊢ subsume_full E L false (l ◁ₗ[π, Owned wl] PlaceIn v @ ◁ value_t (UntypedSynType ly1)) (l ◁ₗ[π, Owned wl] PlaceIn r @ (◁ ty)) T.
+  Proof.
+    iIntros "HT".
+    iIntros (???) "#CTX #HE HL Hl".
+    iMod ("HT" with "[//] [//] CTX HE HL") as "(%L' & % & %R & >(Hv & HR) & HL & % & % & HT)".
+    iPoseProof (ofty_own_merge_value with "Hv Hl") as "?"; first done.
+    iModIntro. iExists L', R. iFrame. done.
+  Qed.
+  (* should have a lower priority than Lithium's id instance - in case the goal specifies that we want a value_t, we should not try to fiddle with that. *)
+  Global Instance subsume_full_value_merge_ofty_untyped_inst {rt} π E L (ty : type rt) r v l ly1 wl :
+    SubsumeFull E L false (l ◁ₗ[π, Owned wl] PlaceIn v @ ◁ value_t (UntypedSynType ly1))%I (l ◁ₗ[π, Owned wl] PlaceIn r @ (◁ ty))%I | 100 :=
+    λ T, i2p (subsume_full_value_merge_ofty_untyped π E L ty r v l ly1 wl T).
 
+  Lemma subsume_full_value_merge_ofty {rt} π E L (ty : type rt) r v l st wl T :
+    (prove_with_subtype E L false ProveDirect (v ◁ᵥ{π} r @ ty) (λ L' _ R,
+      ⌜ty.(ty_has_op_type) (use_op_alg' ty.(ty_syn_type)) MCCopy⌝ ∗ ⌜ty_syn_type ty = st⌝ ∗ T L' R))
+    ⊢ subsume_full E L false (l ◁ₗ[π, Owned wl] #v @ ◁ value_t st) (l ◁ₗ[π, Owned wl] #r @ (◁ ty)) T.
+  Proof.
+    iIntros "HT".
+    iIntros (???) "#CTX #HE HL Hl". iPoseProof (ltype_own_has_layout with "Hl") as "(%ly' & %Hst & %)".
+    iMod ("HT" with "[//] [//] CTX HE HL") as "(%L' & % & %R & >(Hv & HR) & HL & %Hc & %Ha & HT)".
+    iModIntro. iExists L', R. iFrame.
+    iApply (ofty_own_merge_value with "Hv Hl").
+    destruct st; try done. simp_ltypes in Hst. simpl in Hst. rewrite Ha.
+    specialize (syn_type_has_layout_untyped_inv _ _ Hst) as (-> & _).
+    rewrite Ha in Hc. split; done.
+  Qed.
+  (* should have a lower priority than Lithium's id instance - in case the goal specifies that we want a value_t, we should not try to fiddle with that. *)
+  Global Instance subsume_full_value_merge_ofty_inst {rt} π E L (ty : type rt) r v l st wl :
+    SubsumeFull E L false (l ◁ₗ[π, Owned wl] PlaceIn v @ ◁ value_t st)%I (l ◁ₗ[π, Owned wl] PlaceIn r @ (◁ ty))%I | 101 :=
+    λ T, i2p (subsume_full_value_merge_ofty π E L ty r v l st wl T).
+
+  Lemma owned_subtype_value_merge {rt} π E L (ty : type rt) r v' st T :
+    prove_with_subtype E L false ProveDirect (v' ◁ᵥ{π} r @ ty) (λ L' _ R,
+      introduce_with_hooks E L' R (λ L2, ⌜ty.(ty_has_op_type) (use_op_alg' ty.(ty_syn_type)) MCCopy⌝ ∗
+      ⌜ty_syn_type ty = st⌝ ∗ T L2))
+    ⊢ owned_subtype π E L false v' r (value_t st) (ty) T.
+  Proof.
+    iIntros "HT".
+    iIntros (???) "#CTX #HE HL".
+    iMod ("HT" with "[//] [//] CTX HE HL") as "(%L2 & %κs & %R & >(Hv' & HR) & HL & HT)".
+    iMod ("HT" with "[//] HE HL HR") as "(%L3 & HL & %Hot & <- & HT)".
+    iExists _. iFrame. iModIntro.
+    iPoseProof (ty_own_val_sidecond with "Hv'") as "#$".
+    iSplitR. { iPureIntro. simpl. iIntros (????). f_equiv. by eapply syn_type_has_layout_inj. }
+    iSplitR; first by eauto.
+    iIntros (v) "Hv".
+    iEval (rewrite /ty_own_val/=) in "Hv".
+    iDestruct "Hv" as "(%ot & %Hot' & %Hmc & %Hly & %Hst')".
+    rewrite /use_op_alg' Hot'/= in Hot.
+    destruct Hmc as [-> | (st & ->)]; first done.
+    iApply (ty_memcast_compat_copy with "Hv'"). done.
+  Qed.
+  (* shouldn't have super high priority because the conclusion is very general *)
+  Global Instance owned_subtype_value_merge_inst {rt} π E L (ty : type rt) r v' st :
+    OwnedSubtype π E L false v' r (value_t st) (ty) | 100 :=
+    λ T, i2p (owned_subtype_value_merge π E L ty r v' st T).
+End rules.
+
+Section unify_loc.
+  Context `{!typeGS Σ}.
   (** Strategy for unifying two values:
      Step 1 (equalize st):
      - if goal st is evar, instantiate with same and proceed to 2
@@ -575,99 +599,6 @@ Section rules.
         c) otherwise (size also not equal), require current to be a prefix and continue with prove_with_subtype of the rest (startign at step 1 again); require goal's alignment to be lower
      - otherwise: require the values to be the same.
    *)
-
-  (** Step 2 *)
-
-  (* if both are using the same st, unify the values *)
-  Lemma subsume_full_ofty_value_unify_vs π E L step l vs1 vs2 st T :
-    ⌜vs1 = vs2⌝ ∗ T L True%I
-    ⊢ subsume_full E L step (l ◁ₗ[π, Owned false] PlaceIn vs1 @ ◁ value_t st) (l ◁ₗ[π, Owned false] PlaceIn vs2 @ ◁ value_t st) T.
-  Proof.
-    iIntros "(-> & HT)". iApply subsume_full_id. done.
-  Qed.
-  Global Instance subsume_full_ofty_value_unify_vs_inst π E L step l vs1 vs2 st :
-    SubsumeFull E L step (l ◁ₗ[π, Owned false] PlaceIn vs1 @ ◁ value_t st)%I (l ◁ₗ[π, Owned false] PlaceIn vs2 @ ◁ value_t st)%I | 5 :=
-    λ T, i2p (subsume_full_ofty_value_unify_vs π E L step l vs1 vs2 st T).
-
-
-
-  (* if both are untyped, and have not been handled by the previous instance,
-     check if the sizes of the layout are the same;
-     - if so, fully subsume the values
-     - else if the size of the first layout is smaller, prove that the left one is a prefix of the latter, and continue searching for the rest.
-     - else, the goal refers to a subset of the current chunk and we split off. *)
-  Lemma subsume_full_ofty_value_untyped_full π E L step l vs1 vs2 ly1 ly2 T `{!LayoutSizeEq ly1 ly2} :
-    (⌜l `has_layout_loc` ly1⌝ -∗ ⌜ly_align_in_bounds ly1⌝ -∗ ⌜l `has_layout_loc` ly2⌝ ∗ ⌜vs1 = vs2⌝ ∗ ⌜ly_align_in_bounds ly2⌝ ∗ ⌜layout_wf ly2⌝ ∗ T L True%I)
-    ⊢ subsume_full E L step (l ◁ₗ[π, Owned false] vs1 @ ◁ value_t (UntypedSynType ly1)) (l ◁ₗ[π, Owned false] vs2 @ ◁ value_t (UntypedSynType ly2)) T.
-  Proof.
-    (*iIntros "(%Halign & -> & HT)".*)
-    iIntros "HT".
-    iIntros (F ??) "#CTX #HE HL Hl". iModIntro. iExists L, True%I. iFrame.
-    iPoseProof (ltype_own_has_layout with "Hl") as "(%ly' & %Hly' & %Hlyl)". simp_ltypes in Hly'. simpl in *.
-    apply syn_type_has_layout_untyped_inv in Hly' as (-> & ? & ? & ?).
-    iPoseProof ("HT" with "[//] [//]") as "(% & -> & % & % & HT)".
-    iPoseProof (ofty_value_t_untyped_reduce_alignment _ _ _ _ ly2 with "Hl") as "Hl".
-    { done. }
-    { done. }
-    { done. }
-    { done. }
-    iFrame. iApply (maybe_logical_step_intro). iL. done.
-  Qed.
-  Global Instance subsume_full_ofty_value_untyped_full_inst π E L step l vs1 vs2 ly1 ly2 `{!LayoutSizeEq ly1 ly2} :
-    SubsumeFull E L step (l ◁ₗ[π, Owned false] vs1 @ ◁ value_t (UntypedSynType ly1))%I (l ◁ₗ[π, Owned false] vs2 @ ◁ value_t (UntypedSynType ly2))%I | 6 :=
-    λ T, i2p (subsume_full_ofty_value_untyped_full π E L step l vs1 vs2 ly1 ly2 T).
-
-
-  (* TODO: need simplification mechanism for the ly_offset here to get to a sane layout.
-    Or more specifically: a SimplifyHyp instance for value_t. *)
-    (*ly_size ly2 = ly_size (ly_offset ly3 (ly_size ly1))*)
-  Lemma subsume_full_ofty_value_untyped_prefix π E L step l vs1 vs2 ly1 ly2 T `{!LayoutSizeLe ly1 ly2} :
-    (⌜syn_type_has_layout (UntypedSynType ly2) ly2⌝ ∗
-    (⌜l `has_layout_loc` ly1⌝ -∗
-    ⌜l `has_layout_loc` ly2⌝ ∗
-    ∃ vs2', ⌜vs2 = vs1 ++ vs2'⌝ ∗
-    ∃ ly1', prove_with_subtype E L step ProveDirect ((l +ₗ ly_size ly1) ◁ₗ[π, Owned false] PlaceIn vs2' @ ◁ value_t (UntypedSynType ly1')) (λ L2 _ R2, ⌜ly_size ly1' = ly_size ly2 - ly_size ly1⌝ ∗ T L2 R2)))
-    ⊢ subsume_full E L step (l ◁ₗ[π, Owned false] #vs1 @ ◁ value_t (UntypedSynType ly1)) (l ◁ₗ[π, Owned false] #vs2 @ ◁ value_t (UntypedSynType ly2)) T.
-  Proof.
-    iIntros "(%Hst & HT)".
-    match goal with H : LayoutSizeLe _ _ |- _ => rewrite /LayoutSizeLe in H end.
-    iIntros (F ??) "#CTX #HE HL Hl".
-    iPoseProof (ltype_own_has_layout with "Hl") as "(%ly & %Halg & %Hal)".
-    apply syn_type_has_layout_untyped_inv in Halg as (-> & ? & ?).
-    iDestruct ("HT" with "[//]") as "(%Hal2 & %vs2' & -> & %ly1' & HT)".
-    iMod ("HT" with "[//] [//] CTX HE HL") as "(%L' & % & %R2 & Hl' & HL & %Hsz & HT)".
-    iExists _, R2. iFrame.
-    iApply maybe_logical_step_fupd.
-    iApply (maybe_logical_step_compose with "Hl'").
-    iApply maybe_logical_step_intro.
-    iIntros "!> (Hl' & $)".
-    iPoseProof (ofty_value_t_merge_adjacent with "Hl Hl'") as "$"; last done.
-    - done.
-    - done.
-    - done.
-    - done.
-  Qed.
-  Global Instance subsume_full_ofty_value_untyped_prefix_inst π E L step l vs1 vs2 ly1 ly2 `{!LayoutSizeLe ly1 ly2} :
-    SubsumeFull E L step (l ◁ₗ[π, Owned false] #vs1 @ ◁ value_t (UntypedSynType ly1))%I (l ◁ₗ[π, Owned false] #vs2 @ ◁ value_t (UntypedSynType ly2))%I | 7 :=
-    λ T, i2p (subsume_full_ofty_value_untyped_prefix π E L step l vs1 vs2 ly1 ly2 T).
-
-  (* TODO we should also have a corresponding case for the thing that the new one is smaller *)
-  (*
-  Lemma subsume_full_ofty_value_untyped_larger π E L step l vs1 vs2 ly1 ly2 T :
-    (⌜ly_size ly2 ≤ ly_size ly1⌝ ∗
-    ⌜ly_align_log ly2 ≤ ly_align_log ly1⌝ ∗
-    ⌜layout_wf (ly_offset ly1 (ly_size ly2))⌝ ∗
-    ⌜vs2 = take (ly_size ly2) vs1⌝ ∗
-    ((l +ₗ ly_size ly2) ◁ₗ[π, Owned false] PlaceIn (drop (ly_size ly2) vs1) @ (◁ value_t (UntypedSynType (ly_offset ly1 (ly_size ly2)))) -∗ T L True%I))-∗
-    subsume_full E L step (l ◁ₗ[π, Owned false] #vs1 @ ◁ value_t (UntypedSynType ly1)) (l ◁ₗ[π, Owned false] #vs2 @ ◁ value_t (UntypedSynType ly2)) T.
-  Proof.
-    (* TODO *)
-  Admitted.
-  Global Instance subsume_full_ofty_value_untyped_larger_inst π E L step l vs1 vs2 ly1 ly2 :
-    SubsumeFull E L step (l ◁ₗ[π, Owned false] PlaceIn vs1 @ ◁ value_t (UntypedSynType ly1))%I (l ◁ₗ[π, Owned false] PlaceIn vs2 @ ◁ value_t (UntypedSynType ly2))%I | 9 :=
-    λ T, i2p (subsume_full_ofty_value_untyped_larger π E L step l vs1 vs2 ly1 ly2 T).
-   *)
-
 
   (** Step 1 *)
   (* instantiate in case [st2] is an evar *)
@@ -727,17 +658,107 @@ Section rules.
     λ T, i2p (subsume_full_ofty_value_st_eq π E L step l vs1 vs2 st1 st2 T).
 
 
-  (** Same instances for the case that we have just values *)
+  (** Step 2 *)
+
   (* if both are using the same st, unify the values *)
-  Lemma subsume_full_value_unify_vs E L step π v vs1 vs2 st T :
+  Lemma subsume_full_ofty_value_unify_vs π E L step l vs1 vs2 st T :
     ⌜vs1 = vs2⌝ ∗ T L True%I
-    ⊢ subsume_full E L step (v ◁ᵥ{π} vs1 @ value_t st) (v ◁ᵥ{π} vs2 @ value_t st) T.
+    ⊢ subsume_full E L step (l ◁ₗ[π, Owned false] #vs1 @ ◁ value_t st) (l ◁ₗ[π, Owned false] #vs2 @ ◁ value_t st) T.
   Proof.
     iIntros "(-> & HT)". iApply subsume_full_id. done.
   Qed.
-  Global Instance subsume_full_value_unify_vs_inst E L step π v vs1 vs2 st :
-    SubsumeFull E L step (v ◁ᵥ{π} vs1 @ value_t st)%I (v ◁ᵥ{π} vs2 @ value_t st)%I | 5 :=
-    λ T, i2p (subsume_full_value_unify_vs E L step π v vs1 vs2 st T).
+  Global Instance subsume_full_ofty_value_unify_vs_inst π E L step l vs1 vs2 st :
+    SubsumeFull E L step (l ◁ₗ[π, Owned false] #vs1 @ ◁ value_t st)%I (l ◁ₗ[π, Owned false] #vs2 @ ◁ value_t st)%I | 5 :=
+    λ T, i2p (subsume_full_ofty_value_unify_vs π E L step l vs1 vs2 st T).
+
+
+  (* if both are untyped, and have not been handled by the previous instance,
+     check if the sizes of the layout are the same;
+     - if so, fully subsume the values
+     - else if the size of the first layout is smaller, prove that the left one is a prefix of the latter, and continue searching for the rest.
+     - else, the goal refers to a subset of the current chunk and we split off. *)
+  Lemma subsume_full_ofty_value_untyped_full π E L step l vs1 vs2 ly1 ly2 T `{!LayoutSizeEq ly1 ly2} :
+    (⌜l `has_layout_loc` ly1⌝ -∗ ⌜ly_align_in_bounds ly1⌝ -∗ ⌜l `has_layout_loc` ly2⌝ ∗ ⌜vs1 = vs2⌝ ∗ ⌜ly_align_in_bounds ly2⌝ ∗ ⌜layout_wf ly2⌝ ∗ T L True%I)
+    ⊢ subsume_full E L step (l ◁ₗ[π, Owned false] vs1 @ ◁ value_t (UntypedSynType ly1))
+        (l ◁ₗ[π, Owned false] vs2 @ ◁ value_t (UntypedSynType ly2)) T.
+  Proof.
+    (*iIntros "(%Halign & -> & HT)".*)
+    iIntros "HT".
+    iIntros (F ??) "#CTX #HE HL Hl". iModIntro. iExists L, True%I. iFrame.
+    iPoseProof (ltype_own_has_layout with "Hl") as "(%ly' & %Hly' & %Hlyl)". simp_ltypes in Hly'. simpl in *.
+    apply syn_type_has_layout_untyped_inv in Hly' as (-> & ? & ? & ?).
+    iPoseProof ("HT" with "[//] [//]") as "(% & -> & % & % & HT)".
+    iPoseProof (ofty_value_untyped_reduce_alignment _ _ _ _ ly2 with "Hl") as "Hl".
+    { done. }
+    { done. }
+    { done. }
+    { done. }
+    iFrame. iApply (maybe_logical_step_intro). iL. done.
+  Qed.
+  Global Instance subsume_full_ofty_value_untyped_full_inst π E L step l vs1 vs2 ly1 ly2 `{!LayoutSizeEq ly1 ly2} :
+    SubsumeFull E L step (l ◁ₗ[π, Owned false] vs1 @ ◁ value_t (UntypedSynType ly1))%I (l ◁ₗ[π, Owned false] vs2 @ ◁ value_t (UntypedSynType ly2))%I | 6 :=
+    λ T, i2p (subsume_full_ofty_value_untyped_full π E L step l vs1 vs2 ly1 ly2 T).
+
+
+  (* Prove a prefix of the goal, and continue finding the rest of the ownership *)
+  Lemma subsume_full_ofty_value_untyped_prefix π E L step l vs1 vs2 ly1 ly2 T `{!LayoutSizeLe ly1 ly2} :
+    (⌜syn_type_has_layout (UntypedSynType ly2) ly2⌝ ∗
+    (⌜l `has_layout_loc` ly1⌝ -∗
+    ⌜l `has_layout_loc` ly2⌝ ∗
+    ∃ vs2', ⌜vs2 = vs1 ++ vs2'⌝ ∗
+    ∃ ly1', prove_with_subtype E L step ProveDirect ((l +ₗ ly_size ly1) ◁ₗ[π, Owned false] #vs2' @ ◁ value_t (UntypedSynType ly1'))
+        (λ L2 _ R2, ⌜ly_size ly1' = ly_size ly2 - ly_size ly1⌝ ∗ T L2 R2)))
+    ⊢ subsume_full E L step (l ◁ₗ[π, Owned false] #vs1 @ ◁ value_t (UntypedSynType ly1))
+        (l ◁ₗ[π, Owned false] #vs2 @ ◁ value_t (UntypedSynType ly2)) T.
+  Proof.
+    iIntros "(%Hst & HT)".
+    match goal with H : LayoutSizeLe _ _ |- _ => rewrite /LayoutSizeLe in H end.
+    iIntros (F ??) "#CTX #HE HL Hl".
+    iPoseProof (ltype_own_has_layout with "Hl") as "(%ly & %Halg & %Hal)".
+    apply syn_type_has_layout_untyped_inv in Halg as (-> & ? & ?).
+    iDestruct ("HT" with "[//]") as "(%Hal2 & %vs2' & -> & %ly1' & HT)".
+    iMod ("HT" with "[//] [//] CTX HE HL") as "(%L' & % & %R2 & Hl' & HL & %Hsz & HT)".
+    iExists _, R2. iFrame.
+    iApply maybe_logical_step_fupd.
+    iApply (maybe_logical_step_compose with "Hl'").
+    iApply maybe_logical_step_intro.
+    iIntros "!> (Hl' & $)".
+    iPoseProof (ofty_value_untyped_app_merge with "Hl Hl'") as "$"; last done.
+    - done.
+    - done.
+    - done.
+    - done.
+  Qed.
+  Global Instance subsume_full_ofty_value_untyped_prefix_inst π E L step l vs1 vs2 ly1 ly2 `{!LayoutSizeLe ly1 ly2} :
+    SubsumeFull E L step (l ◁ₗ[π, Owned false] #vs1 @ ◁ value_t (UntypedSynType ly1))%I (l ◁ₗ[π, Owned false] #vs2 @ ◁ value_t (UntypedSynType ly2))%I | 7 :=
+    λ T, i2p (subsume_full_ofty_value_untyped_prefix π E L step l vs1 vs2 ly1 ly2 T).
+
+  (* TODO we should also have a corresponding case if the RHS is smaller *)
+  (* TODO: need simplification mechanism for the ly_offset here to get to a sane layout.
+    Or more specifically: a SimplifyHyp instance for value_t. *)
+    (*ly_size ly2 = ly_size (ly_offset ly3 (ly_size ly1))*)
+  (*
+  Lemma subsume_full_ofty_value_untyped_larger π E L step l vs1 vs2 ly1 ly2 T :
+    (⌜ly_size ly2 ≤ ly_size ly1⌝ ∗
+    ⌜ly_align_log ly2 ≤ ly_align_log ly1⌝ ∗
+    ⌜layout_wf (ly_offset ly1 (ly_size ly2))⌝ ∗
+    ⌜vs2 = take (ly_size ly2) vs1⌝ ∗
+    ((l +ₗ ly_size ly2) ◁ₗ[π, Owned false] PlaceIn (drop (ly_size ly2) vs1) @ (◁ value_t (UntypedSynType (ly_offset ly1 (ly_size ly2)))) -∗ T L True%I))-∗
+    subsume_full E L step (l ◁ₗ[π, Owned false] #vs1 @ ◁ value_t (UntypedSynType ly1)) (l ◁ₗ[π, Owned false] #vs2 @ ◁ value_t (UntypedSynType ly2)) T.
+  Proof.
+    (* TODO *)
+  Admitted.
+  Global Instance subsume_full_ofty_value_untyped_larger_inst π E L step l vs1 vs2 ly1 ly2 :
+    SubsumeFull E L step (l ◁ₗ[π, Owned false] PlaceIn vs1 @ ◁ value_t (UntypedSynType ly1))%I (l ◁ₗ[π, Owned false] PlaceIn vs2 @ ◁ value_t (UntypedSynType ly2))%I | 9 :=
+    λ T, i2p (subsume_full_ofty_value_untyped_larger π E L step l vs1 vs2 ly1 ly2 T).
+   *)
+End unify_loc.
+
+Section unify_val.
+  Context `{!typeGS Σ}.
+
+  (** Same instances for the case that we have just values *)
+
 
   (* if both are untyped, and have not been handled by the previous instance,
      check if the sizes of the layout are the same;
@@ -758,23 +779,6 @@ Section rules.
     λ T, i2p (subsume_full_ofty_value_untyped_prefix π E L l vs1 vs2 ly1 ly2 T).
    *)
 
-  Lemma subsume_full_value_untyped_full π E L step v vs1 vs2 ly1 ly2 T `{!LayoutSizeEq ly1 ly2} :
-    ⌜ly_align_log ly2 ≤ ly_align_log ly1⌝ ∗ ⌜vs1 = vs2⌝ ∗ T L True%I
-    ⊢ subsume_full E L step (v ◁ᵥ{π} vs1 @ value_t (UntypedSynType ly1)) (v ◁ᵥ{π} vs2 @ value_t (UntypedSynType ly2)) T.
-  Proof.
-    iIntros "(%Hal & -> & HT)".
-    iIntros (???) "#CTX #HE HL Hv".
-    iExists _, _. iFrame.
-    iApply maybe_logical_step_intro. iL.
-    iApply value_untyped_mono; last done.
-    - done.
-    - intros. by eapply layout_wf_mono.
-    - intros. by eapply ly_align_in_bounds_mono.
-  Qed.
-  (* NOTE: needs to be higher-priority than [subsume_full_value_st_untyped] in order to prevent divergence *)
-  Global Instance subsume_full_value_untyped_full_inst π E L step v vs1 vs2 ly1 ly2 `{!LayoutSizeEq ly1 ly2} :
-    SubsumeFull E L step (v ◁ᵥ{π} vs1 @ value_t (UntypedSynType ly1))%I (v ◁ᵥ{π} vs2 @ value_t (UntypedSynType ly2))%I | 6 :=
-    λ T, i2p (subsume_full_value_untyped_full π E L step v vs1 vs2 ly1 ly2 T).
 
   (** Step 1 *)
   (* instantiate in case [st2] is an evar *)
@@ -799,7 +803,7 @@ Section rules.
     iMod ("HT" with "[//] [//] CTX HE HL Hv") as "(%L2 & %R2 & Hv & ? & ?)".
     iExists L2, _. iFrame.
     iApply (maybe_logical_step_wand with "[] Hv").
-    iIntros "(Hv & $)". iApply value_make_typed; done.
+    iIntros "(Hv & $)". iApply value_untyped_make_typed; done.
   Qed.
   Global Instance subsume_full_value_st_untyped_inst E L step π v ly1 st2 vs1 vs2 :
     SubsumeFull E L step (v ◁ᵥ{π} vs1 @ value_t (UntypedSynType ly1))%I (v ◁ᵥ{π} vs2 @ value_t st2)%I | 15 :=
@@ -817,304 +821,50 @@ Section rules.
     SubsumeFull E L step (v ◁ᵥ{π} vs1 @ value_t st1)%I (v ◁ᵥ{π} vs2 @ value_t st2)%I | 20 :=
     λ T, i2p (subsume_full_value_st_eq E L step π v vs1 vs2 st1 st2 T).
 
-
-
   (* TODO: one thing that definitely needs to work:
       value_t (UntypedOp ly) <: value_t st when st_has_layout st ly
    *)
 
-
-  (* When we require assembled ownership, try to assemble it. *)
-  (* This needs to have lower priority than the above subsumption instances that specialize to the case where [ty = value_t _]. *)
-  (* In addition, other rules for other types should similarly be able to implement their own proof strategies.
-     Namely, this rule makes a pretty strong commitment (having an exactly fitting value assignment available),
-      so we should really try it as a last resort. So we give it a pretty low priority.
-   *)
-  (* TODO: for this, need some ty_has_syn_type relation that also captures the Untyped case *)
-  (* TODO ideally, the requirement for the UntypedOp case should just generally hold for types. Untyped should always be possible. *)
-  Lemma subsume_value_merge_ofty {rt} π (ty : type rt) r v l st wl T :
-    (v ◁ᵥ{π} r @ ty ∗
-      ⌜match st with
-      | UntypedSynType ly1 => syn_type_has_layout ty.(ty_syn_type) ly1 ∧ ty_has_op_type ty (UntypedOp ly1) MCCopy
-      | _ => ty.(ty_has_op_type) (use_op_alg' ty.(ty_syn_type)) MCCopy ∧ ty_syn_type ty = st
-      end⌝ ∗ T)
-    ⊢ subsume (l ◁ₗ[π, Owned wl] PlaceIn v @ ◁ value_t st) (l ◁ₗ[π, Owned wl] PlaceIn r @ (◁ ty)) T.
+  (** Step 2 *)
+  (* for untyped, require compatibility of the layouts *)
+  Lemma subsume_full_value_untyped_full π E L step v vs1 vs2 ly1 ly2 T `{!LayoutSizeEq ly1 ly2} :
+    ⌜ly_align_log ly2 ≤ ly_align_log ly1⌝ ∗ ⌜vs1 = vs2⌝ ∗ T L True%I
+    ⊢ subsume_full E L step (v ◁ᵥ{π} vs1 @ value_t (UntypedSynType ly1)) (v ◁ᵥ{π} vs2 @ value_t (UntypedSynType ly2)) T.
   Proof.
-    iDestruct 1 as "(Hv & %Ha & HT)". simpl.
-    iIntros "Hl".
-    rewrite !ltype_own_ofty_unfold /lty_of_ty_own.
-    iDestruct "Hl" as "(%ly & %Halg & % & Hsc & Hlb & Hcred & %r' & Hrfn & Hb)".
-    simpl in Halg. iFrame "HT".
-    iExists ly.
-    iFrame. iFrame "%".
-    iPoseProof (ty_own_val_sidecond with "Hv") as "#$".
-    assert ((∃ ly1, st = UntypedSynType ly1 ∧ syn_type_has_layout (ty_syn_type ty) ly1 ∧ ty_has_op_type ty (UntypedOp ly1) MCCopy) ∨ (ty_has_op_type ty (use_op_alg' (ty_syn_type ty)) MCCopy ∧ ty_syn_type ty = st)) as Hb.
-    { destruct st; eauto. }
-    iSplitR. { iPureIntro. destruct Hb as [(ly1 & -> & ? & ?) | (? & <-)]; last done.
-      apply syn_type_has_layout_untyped_inv in Halg as (-> & _). done. }
-    iExists r. iSplitR; first done.
-    iNext. iMod "Hb" as "(%v' & Hl & Hv')". iModIntro.
-    iDestruct "Hrfn" as "<-".
-    iExists v'. iFrame.
-    iEval (rewrite /ty_own_val/=) in "Hv'".
-    iDestruct "Hv'" as "(%ot & %Hot' & %Hmc & %Hv & ?)".
-    destruct Hmc as [-> | [st' ->]]; first done.
-    iApply (ty_memcast_compat_copy with "Hv").
-
-    destruct Hb as [(ly1 & -> & Hst & ?) | (Hst & <-)].
-    - injection Hot' as <-. done.
-    - move: Hst. rewrite /use_op_alg' Hot' //.
-  Qed.
-
-  Lemma subsume_full_value_merge_ofty_untyped {rt} π E L (ty : type rt) r v l ly1 wl T :
-    (prove_with_subtype E L false ProveDirect (v ◁ᵥ{π} r @ ty) (λ L' _ R,
-      ⌜syn_type_has_layout ty.(ty_syn_type) ly1⌝ ∗ ⌜ty_has_op_type ty (UntypedOp ly1) MCCopy⌝ ∗ T L' R))
-    ⊢ subsume_full E L false (l ◁ₗ[π, Owned wl] PlaceIn v @ ◁ value_t (UntypedSynType ly1)) (l ◁ₗ[π, Owned wl] PlaceIn r @ (◁ ty)) T.
-  Proof.
-    iIntros "HT".
-    iIntros (???) "#CTX #HE HL Hl".
-    iMod ("HT" with "[//] [//] CTX HE HL") as "(%L' & % & %R & >(Hv & HR) & HL & % & % & HT)".
-    iModIntro. iExists L', R. iFrame.
-    iPoseProof (subsume_value_merge_ofty _ _ _ _ _ _ _ True%I with "[$Hv ] Hl") as "($ & _)"; last done.
-    iL. done.
-  Qed.
-  (* should have a lower priority than Lithium's id instance - in case the goal specifies that we want a value_t, we should not try to fiddle with that. *)
-  Global Instance subsume_full_value_merge_ofty_untyped_inst {rt} π E L (ty : type rt) r v l ly1 wl :
-    SubsumeFull E L false (l ◁ₗ[π, Owned wl] PlaceIn v @ ◁ value_t (UntypedSynType ly1))%I (l ◁ₗ[π, Owned wl] PlaceIn r @ (◁ ty))%I | 100 :=
-    λ T, i2p (subsume_full_value_merge_ofty_untyped π E L ty r v l ly1 wl T).
-
-  Lemma subsume_full_value_merge_ofty {rt} π E L (ty : type rt) r v l st wl T :
-    (prove_with_subtype E L false ProveDirect (v ◁ᵥ{π} r @ ty) (λ L' _ R,
-      ⌜ty.(ty_has_op_type) (use_op_alg' ty.(ty_syn_type)) MCCopy⌝ ∗ ⌜ty_syn_type ty = st⌝ ∗ T L' R))
-    ⊢ subsume_full E L false (l ◁ₗ[π, Owned wl] PlaceIn v @ ◁ value_t st) (l ◁ₗ[π, Owned wl] PlaceIn r @ (◁ ty)) T.
-  Proof.
-    iIntros "HT".
-    iIntros (???) "#CTX #HE HL Hl". iPoseProof (ltype_own_has_layout with "Hl") as "(%ly' & %Hst & %)".
-    iMod ("HT" with "[//] [//] CTX HE HL") as "(%L' & % & %R & >(Hv & HR) & HL & %Hc & %Ha & HT)".
-    iModIntro. iExists L', R. iFrame.
-    iPoseProof (subsume_value_merge_ofty _ _ _ _ _ _ _ True%I with "[$Hv] Hl") as "($ & _)"; last done.
-    iL. destruct st; try done. simp_ltypes in Hst. simpl in Hst. rewrite Ha.
-    specialize (syn_type_has_layout_untyped_inv _ _ Hst) as (-> & _).
-    rewrite Ha in Hc. iPureIntro. split; done.
-  Qed.
-  (* should have a lower priority than Lithium's id instance - in case the goal specifies that we want a value_t, we should not try to fiddle with that. *)
-  Global Instance subsume_full_value_merge_ofty_inst {rt} π E L (ty : type rt) r v l st wl :
-    SubsumeFull E L false (l ◁ₗ[π, Owned wl] PlaceIn v @ ◁ value_t st)%I (l ◁ₗ[π, Owned wl] PlaceIn r @ (◁ ty))%I | 101 :=
-    λ T, i2p (subsume_full_value_merge_ofty π E L ty r v l st wl T).
-
-  Lemma owned_subtype_value_merge {rt} π E L (ty : type rt) r v' st T :
-    prove_with_subtype E L false ProveDirect (v' ◁ᵥ{π} r @ ty) (λ L' _ R,
-      introduce_with_hooks E L' R (λ L2, ⌜ty.(ty_has_op_type) (use_op_alg' ty.(ty_syn_type)) MCCopy⌝ ∗
-      ⌜ty_syn_type ty = st⌝ ∗ T L2))
-    ⊢ owned_subtype π E L false v' r (value_t st) (ty) T.
-  Proof.
-    iIntros "HT".
-    iIntros (???) "#CTX #HE HL".
-    iMod ("HT" with "[//] [//] CTX HE HL") as "(%L2 & %κs & %R & >(Hv' & HR) & HL & HT)".
-    iMod ("HT" with "[//] HE HL HR") as "(%L3 & HL & %Hot & <- & HT)".
-    iExists _. iFrame. iModIntro.
-    iPoseProof (ty_own_val_sidecond with "Hv'") as "#$".
-    iSplitR. { iPureIntro. simpl. iIntros (????). f_equiv. by eapply syn_type_has_layout_inj. }
-    iSplitR; first by eauto.
-    iIntros (v) "Hv".
-    iEval (rewrite /ty_own_val/=) in "Hv".
-    iDestruct "Hv" as "(%ot & %Hot' & %Hmc & %Hly & %Hst')".
-    rewrite /use_op_alg' Hot'/= in Hot.
-    destruct Hmc as [-> | (st & ->)]; first done.
-    iApply (ty_memcast_compat_copy with "Hv'"). done.
-  Qed.
-  (* shouldn't have super high priority because the conclusion is very general *)
-  Global Instance owned_subtype_value_merge_inst {rt} π E L (ty : type rt) r v' st :
-    OwnedSubtype π E L false v' r (value_t st) (ty) | 100 :=
-    λ T, i2p (owned_subtype_value_merge π E L ty r v' st T).
-  (*
-  Lemma subsume_full_value_merge {rt} π E L (ty : type rt) r v v' st T :
-    prove_with_subtype E L false ProveDirect (v' ◁ᵥ{π} r @ ty) (λ L' _ R,
-      ⌜ty.(ty_has_op_type) (use_op_alg' ty.(ty_syn_type)) MCCopy⌝ ∗ ⌜ty_syn_type ty = st⌝ ∗ T L' R) -∗
-    subsume_full E L false (v ◁ᵥ{π} v' @ value_t st) (v ◁ᵥ{π} r @ ty) T.
-  Proof.
-    iIntros "HT".
+    iIntros "(%Hal & -> & HT)".
     iIntros (???) "#CTX #HE HL Hv".
-    iMod ("HT" with "[//] [//] CTX HE HL") as "(%L2 & %κs & %R & >(Hv' & HR) & HL & %Hot & <- & HT)".
-    iExists _, _. iFrame. iModIntro.
-    iEval (rewrite /ty_own_val/=) in "Hv".
-    iDestruct "Hv" as "(%ot & %Hot' & %Hmc & %Hly & %Hst')".
-    rewrite /use_op_alg' Hot'/= in Hot.
-    destruct Hmc as [-> | (st & ->)]; first done.
-    iApply (ty_memcast_compat_copy with "Hv'"). done.
+    iExists _, _. iFrame.
+    iApply maybe_logical_step_intro. iL.
+    iApply value_untyped_layout_mono; last done.
+    - done.
+    - intros. by eapply layout_wf_mono.
+    - intros. by eapply ly_align_in_bounds_mono.
   Qed.
-   *)
+  (* NOTE: needs to be higher-priority than [subsume_full_value_st_untyped] in order to prevent divergence *)
+  Global Instance subsume_full_value_untyped_full_inst π E L step v vs1 vs2 ly1 ly2 `{!LayoutSizeEq ly1 ly2} :
+    SubsumeFull E L step (v ◁ᵥ{π} vs1 @ value_t (UntypedSynType ly1))%I (v ◁ᵥ{π} vs2 @ value_t (UntypedSynType ly2))%I | 6 :=
+    λ T, i2p (subsume_full_value_untyped_full π E L step v vs1 vs2 ly1 ly2 T).
 
-
-
-  (* Simplification instance - when introducing a value_t, we simply destruct it *)
-  (* TODO how does this overlap with ghost_drop?
-     TODO can we simplify the is_memcast_val? Otherwise, it seems pretty useless. *)
-  (*
-  Lemma value_simplify π v T ot st p :
-    (⌜is_memcast_val p ot v⌝ -∗ ⌜v `has_layout_val` ot_layout ot⌝ -∗ ⌜syn_type_has_layout st (ot_layout ot)⌝ -∗ T) -∗
-    simplify_hyp (v ◁ᵥ{π} p @ value_t st)%I T.
-  Proof. iIntros "HT (% & % & %)". by iApply "HT". Qed.
-  Global Instance value_simplify_inst π v ot st p :
-    SimplifyHypVal v π (value_t ot st) p (Some 0%N) :=
-    λ T, i2p (value_simplify π v T ot st p).
-   *)
-
-  (* We also need stratification instances.
-    - One option: always cancel value_t in stratification.
-        This limits expressivity a bit for specs, because when we really want to have value_t there, we get stuck.
-      => do this for now, it should suffice.
-     - Other option: have a (non-semantic) guidance parameter that gets provided by OpenedLtype.
-       Only if that guidance parameter is not giving us identity do we fold the value_t.
-     - Other option: do not let stratify do this, but rather have subtyping do this before folding.
-
-     TODO: currently not an instance, because we sometimes do not want to do this!
-     Instead, should give stratify some syntactic guidance from OpenedLtype above it.
-   *)
-  Lemma stratify_ltype_ofty_value_owned π E L mu mdu ma {M} (m : M) l st v wl (T : stratify_ltype_cont_t) :
-    find_in_context (FindVal v π) (λ '(existT rt (ty', r')),
-      ⌜ty'.(ty_has_op_type) (use_op_alg' ty'.(ty_syn_type)) MCCopy⌝ ∗
-      ⌜ty'.(ty_syn_type) = st⌝ ∗
-      stratify_ltype π E L mu mdu ma m l (◁ ty') (PlaceIn r') (Owned wl) T)
-    ⊢ stratify_ltype π E L mu mdu ma m l (◁ value_t st)%I (PlaceIn v) (Owned wl) T.
+  (* if both are using the same st, unify the values *)
+  Lemma subsume_full_value_unify_vs E L step π v vs1 vs2 st T :
+    ⌜vs1 = vs2⌝ ∗ T L True%I
+    ⊢ subsume_full E L step (v ◁ᵥ{π} vs1 @ value_t st) (v ◁ᵥ{π} vs2 @ value_t st) T.
   Proof.
-    iDestruct 1 as ([rt [ty' r']]) "(Hv & %Hot & %Heq & HT)" => /=.
-    iIntros (???) "#CTX #HE HL Hl".
-    iPoseProof (ltype_own_has_layout with "Hl") as "#(%ly & %Hst &_)".
-    iPoseProof (subsume_value_merge_ofty with "[$Hv] Hl") as "(Ha & _)".
-    { instantiate (1 := True%I). iSplitR; last done.
-      iPureIntro. subst st. destruct (ty_syn_type ty'); try done.
-      simp_ltypes in Hst. simpl in Hst.
-      specialize (syn_type_has_layout_untyped_inv _ _ Hst) as (-> & _).
-      done. }
-    iMod ("HT" with "[//] [//] CTX HE HL Ha") as "Ha".
-    subst st. eauto.
+    iIntros "(-> & HT)". iApply subsume_full_id. done.
   Qed.
-  (* needs to have a higher priority than the ofty_resolve_ghost instance *)
-  (*Global Instance stratify_ltype_unblock_ofty_value_owned_inst π E L mu mdu ma l st v wl :*)
-    (*StratifyLtype π E L mu mdu ma StratifyUnblockOp l (◁ value_t st)%I (PlaceIn v) (Owned wl) | 10:=*)
-    (*λ T, i2p (stratify_ltype_ofty_value_owned π E L mu mdu ma StratifyUnblockOp l st v wl T).*)
-  (* TODO: not an instance right now since we don't always want to stratify this -- esp. not for functions passing values in their interface *)
+  Global Instance subsume_full_value_unify_vs_inst E L step π v vs1 vs2 st :
+    SubsumeFull E L step (v ◁ᵥ{π} vs1 @ value_t st)%I (v ◁ᵥ{π} vs2 @ value_t st)%I | 5 :=
+    λ T, i2p (subsume_full_value_unify_vs E L step π v vs1 vs2 st T).
 
-  (* TODO: this is now problematic. Maybe should have an untyped bit after all?
-       Alternative: use syn_type_compat everywhere to allow untyped interaction.
+  (* TODO prefix /suffix *)
+End unify_val.
 
-       Use an untyped bit:
-       - then we still have a problem that often we should maybe be talking about a concrete layout instead.
-          In particular when we assemble chunks.
-          For array, we can work around that, since it is "chunkable", but for everything else, that does not really work.
-          Q: do we reallyneed that for anything but arrays?
-          + when we want to have a view on data and change the element type: e.g. in copy_nonoverlapping, would like to have an array of u8.
-            We could in principle also do that for the ArraySynType, but it would be more of a hassle, and we would again end up with a different syntype
-            OTOH is copy_nonoverlapping that much of a concern?
-            In principle, we could also have something that first adapts
-       - making things untyped would be much less of a hassle in the rules.
+Section rules.
+  Context `{!typeGS Σ}.
 
-       Make rules compatible with UntypedSynType everywhere:
-       - what is the intuitive justification for this? Why should we do it?
-         + to my mind, UntypedSynType is just an undesirable artifact -- at least in safe Rust.
-         + for unsafe stuff, the story may be different. We may want to treat stuff just as bytes.
-            - allocation API itself should maybe treat it that way. We should just have some layout there.
-              In our system, we will have a mixed concrete-symbolic layout.
-              Arguably, that should not be a proper syntype, but that's how it is: our types need a syntype, and generally that requirement seems sensible.
-
-       Alternative for this particular issue:
-       - at the place, just don't leave an Untyped, but the right type. We should not loose information there!
-         Then we also do not need a syntype update.
-
-     *)
-
-  (* TODO: consider whether we need special instances for reading/writing.
-     In particular, what if we read with an ot from an UntypedOp-value? Then we should specialize the ot further in the result of the read.
-     - problem currently: the generic ofty instance requires the type to have the same ot
-     - but in case of value_t, we can change the ot!
-
-   *)
-
-
-  (* [type_read_end] instance that does a move -- should be triggered when the copy instance does not work, hence the lower priority.
-     This leaves a [value_t] at the place.
-  *)
-  Lemma type_read_ofty_move_owned_value E L {rt} π (T : typed_read_end_cont_t rt) l (ty : type rt) r ot wl bmin :
-    ( ⌜use_op_alg (ty_syn_type ty) = Some ot⌝ ∗ (* TODO too strong, should also allow Untyped *)
-    (* TODO for some reason, [simpl] will even unfold [ty_has_op_type] here... this breaks automation ofc *)
-      (*⌜ty_allows_reads ty⌝ ∗*)
-      ⌜ty_has_op_type ty (use_op_alg' (ty_syn_type ty)) MCCopy⌝ ∗
-      (*⌜ty.(ty_has_op_type) ot MCCopy⌝ ∗*)
-      ∀ v v', v ◁ᵥ{π} r @ ty -∗
-      T L v' _ (value_t ty.(ty_syn_type)) v val (◁ value_t ty.(ty_syn_type)) (#v) ResultStrong)
-    ⊢ typed_read_end π E L l (◁ ty) (#r) (Owned wl) bmin AllowStrong ot T.
-  Proof.
-    iIntros "(%Hotalg & %Hot & Hs)" (F ???) "#CTX #HE HL Hna".
-    iIntros "_ Hb".
-    iPoseProof (ofty_ltype_acc_owned with "Hb") as "(%ly & %Halg & %Hly & Hsc & Hlb & >(%v & Hl & Hv & Hcl))"; first done.
-    iPoseProof (ty_own_val_has_layout with "Hv") as "%Hlyv"; first done.
-    specialize (ty_op_type_stable Hot) as Halg''.
-    rewrite /use_op_alg' Hotalg in Halg''.
-    assert (ly = ot_layout ot) as ->. { by eapply syn_type_has_layout_inj. }
-    iModIntro. iExists _, _, rt, _, _.
-    iFrame "Hl Hv".
-    iSplitR; first done. iSplitR; first done.
-    iApply (logical_step_wand with "Hcl").
-    iIntros "Hcl %st Hl Hv".
-    iAssert (v ◁ᵥ{π} v @ value_t ty.(ty_syn_type))%I as "Hv'".
-    { rewrite /ty_own_val/=.
-      (*destruct (syn_type_has_layout_op_alg _ _ Halg) as (ot' & Hop & Hot').*)
-      iExists (ot).
-      iR. iSplitR. { iPureIntro. left. done. }
-      iSplitR; last done. iPureIntro. rewrite /has_layout_val . done. }
-    iPoseProof (ty_memcast_compat_copy _ _ _ ot _ st with "Hv'") as "Hv''".
-    { simpl. exists ot. split_and!; first done; last done. by apply is_value_ot_core_refl. }
-    iMod ("Hcl" $! v _ (value_t ty.(ty_syn_type)) (v) with "Hl [//] [] []") as "Hl".
-    { simpl. done. }
-    { iNext. done. }
-    (*iPoseProof (ty_memcast_compat with "Hv") as "Hid"; first done. simpl.*)
-    iModIntro. iExists _, _, (value_t (ty_syn_type ty)), _. iFrame "∗ #".
-    (* strong update *)
-    iExists _, _, _, ResultStrong. iFrame.
-    do 2 iR.
-    iApply "Hs". done.
-  Qed.
-  (* TODO replace the succeeding instances with this, once we have fixed:
-      (a) owned_subtype to be able to move stuff into it again reliably, also below structs etc.
-      (b) the model to allow syntype updates as long as the layout stays the same *)
-  (*Global Instance type_read_ofty_move_owned_inst E L {rt} π wl bmin l (ty : type rt) r ot :*)
-    (*TypedReadEnd π E L l (◁ ty)%I (PlaceIn r) (Owned wl) bmin AllowStrong ot | 19 :=*)
-    (*λ T, i2p (type_read_ofty_move_owned E L π T l ty r ot wl bmin).*)
-
-  (* TODO for Untyped, we currently cannot leave a value, because we cannot do syntype updates, but [value_t] relies on the syntype to compute the value update *)
-  Lemma type_read_ofty_move_owned_value_untyped E L {rt} π (T : typed_read_end_cont_t rt) l (ty : type rt) r ly wl bmin :
-    (⌜ty.(ty_has_op_type) (UntypedOp ly) MCCopy⌝ ∗
-        ∀ v, T L v _ ty r unit (◁ uninit ty.(ty_syn_type)) (#()) ResultStrong)
-    ⊢ typed_read_end π E L l (◁ ty) (#r) (Owned wl) bmin AllowStrong (UntypedOp ly) T.
-  Proof.
-    iIntros "(%Hot & Hs)" (F ???) "#CTX #HE HL Hna".
-    iIntros "_ Hb".
-    iPoseProof (ofty_ltype_acc_owned with "Hb") as "(%ly' & %Halg & %Hly & Hsc & Hlb & >(%v & Hl & Hv & Hcl))"; first done.
-    iPoseProof (ty_own_val_has_layout with "Hv") as "%Hlyv"; first done.
-    specialize (ty_op_type_stable Hot) as Halg''.
-    assert (ly' = ly) as ->. { by eapply syn_type_has_layout_inj. }
-    iModIntro. iExists _, _, rt, _, _.
-    iFrame "Hl Hv".
-    iSplitR; first done. iSplitR; first done.
-    iApply (logical_step_wand with "Hcl").
-    iIntros "Hcl %st Hl Hv". iMod ("Hcl" $! v _ (uninit ty.(ty_syn_type)) tt with "Hl [//] [] []") as "Hl".
-    { simpl. done. }
-    { iNext. iApply uninit_own_spec. iExists _. iSplitR; first done. done. }
-    iPoseProof (ty_memcast_compat with "Hv") as "Hid"; first done. simpl.
-    iModIntro. iExists _, _,_, _. iFrame.
-    (* strong update *)
-    iExists _, _, _, ResultStrong. iFrame.
-    iSplitR; first done.
-    iR.
-    done.
-  Qed.
-  (*
-  Global Instance type_read_ofty_move_owned_untyped_inst E L {rt} π wl bmin l (ty : type rt) r ly :
-    TypedReadEnd π E L l (◁ ty)%I (PlaceIn r) (Owned wl) bmin AllowStrong (UntypedOp ly) | 20 :=
-    λ T, i2p (type_read_ofty_move_owned_untyped E L π T l ty r ly wl bmin).
-  *)
-
+  (* Read instance that leaves uninit on moves.
+     TODO: Ideally, we would like to leave a value instead to not loose information.
+      The lemmas below explore this, but currently do not work. *)
   Lemma type_read_ofty_move_owned E L {rt} π (T : typed_read_end_cont_t rt) l (ty : type rt) r ot wl bmin :
     (⌜ty.(ty_has_op_type) ot MCCopy⌝ ∗
         ∀ v, T L v _ ty r unit (◁ uninit ty.(ty_syn_type)) (#()) ResultStrong)
@@ -1144,50 +894,6 @@ Section rules.
   Global Instance type_read_ofty_move_owned_inst E L {rt} π wl bmin l (ty : type rt) r ot :
     TypedReadEnd π E L l (◁ ty)%I (PlaceIn r) (Owned wl) bmin AllowStrong (ot) | 20 :=
     λ T, i2p (type_read_ofty_move_owned E L π T l ty r ot wl bmin).
-
-  (*
-  Lemma type_read_ofty_move_owned_untyped E L {rt} π (T : typed_read_end_cont_t rt) l (ty : type rt) r ly wl bmin :
-    ( ⌜ty.(ty_has_op_type) (UntypedOp ly) MCCopy⌝ ∗
-      ∀ v v', v ◁ᵥ{π} r @ ty -∗
-      T L v' _ (value_t (UntypedSynType ly)) v val (◁ value_t (UntypedSynType ly)) (#v) ResultStrong) -∗
-      typed_read_end π E L l (◁ ty) (#r) (Owned wl) bmin AllowStrong (UntypedOp ly) T.
-  Proof.
-    iIntros "(%Hot & Hs)" (F ???) "#CTX #HE HL".
-    iIntros "_ Hb".
-    iPoseProof (ofty_ltype_acc_owned with "Hb") as "(%ly' & %Halg & %Hly & Hsc & Hlb & >(%v & Hl & Hv & Hcl))"; first done.
-    iPoseProof (ty_own_val_has_layout with "Hv") as "%Hlyv"; first done.
-    specialize (ty_op_type_stable Hot) as Halg''.
-    (*rewrite /use_op_alg' Hotalg in Halg''.*)
-    assert (ly' = ly) as ->. { by eapply syn_type_has_layout_inj. }
-    iModIntro. iExists _, _, rt, _, _.
-    iFrame "Hl Hv".
-    iSplitR; first done. iSplitR; first done.
-    iApply (logical_step_wand with "Hcl").
-    iIntros "Hcl %st Hl Hv".
-    iAssert (v ◁ᵥ{π} v @ value_t (UntypedSynType ly))%I as "Hv'".
-    { rewrite /ty_own_val/=.
-      (*destruct (syn_type_has_layout_op_alg _ _ Halg) as (ot' & Hop & Hot').*)
-      iExists (UntypedOp ly).
-      iR. iSplitR. { iPureIntro. left. done. }
-      simpl. iR. iPureIntro. by eapply syn_type_has_layout_make_untyped. }
-    (*iPoseProof (ty_memcast_compat_copy _ _ _ ot _ st with "Hv'") as "Hv''".*)
-    (*{ simpl. exists ot. split_and!; first done; last done. by apply is_value_ot_core_refl. }*)
-    iMod ("Hcl" $! v _ (value_t (UntypedSynType ly)) (v) with "Hl [//] [] []") as "Hl".
-    { simpl. done. }
-    { iNext. done. }
-    (*iPoseProof (ty_memcast_compat with "Hv") as "Hid"; first done. simpl.*)
-    iModIntro. iExists _, _, (value_t (ty_syn_type ty)), _. iFrame "∗ #".
-    (* strong update *)
-    iExists _, _, _, ResultStrong. iFrame.
-    do 2 iR.
-    iApply "Hs". done.
-  Qed.
-  Global Instance type_read_ofty_move_owned_inst E L {rt} π wl bmin l (ty : type rt) r ot :
-    TypedReadEnd π E L l (◁ ty)%I (PlaceIn r) (Owned wl) bmin AllowStrong ot | 20 :=
-    λ T, i2p (type_read_ofty_move_owned E L π T l ty r ot wl bmin).
-  *)
-
-
 
   (* We also have a corresponding rule for Uniq ownership that leaves [Opened].
     This allows us to move out of mutable references, as long as another object is moved in at a later point. *)
@@ -1232,6 +938,186 @@ Section rules.
   Global Instance type_read_ofty_move_uniq_inst E L {rt} π κ γ bmin l (ty : type rt) r ot :
     TypedReadEnd π E L l (◁ ty)%I (#r) (Uniq κ γ) bmin AllowStrong ot | 20 :=
     λ T, i2p (type_read_ofty_move_uniq E L π T l ty r ot κ γ bmin).
+
+  (* [type_read_end] instance that does a move -- should be triggered when the copy instance does not work, hence the lower priority.
+     This leaves a [value_t] at the place. *)
+  Lemma type_read_ofty_move_owned_value E L {rt} π (T : typed_read_end_cont_t rt) l (ty : type rt) r ot wl bmin :
+    ( ⌜use_op_alg (ty_syn_type ty) = Some ot⌝ ∗ (* TODO too strong, should also allow Untyped *)
+    (* TODO for some reason, [simpl] will even unfold [ty_has_op_type] here... this breaks automation ofc *)
+      (*⌜ty_allows_reads ty⌝ ∗*)
+      ⌜ty_has_op_type ty (use_op_alg' (ty_syn_type ty)) MCCopy⌝ ∗
+      (*⌜ty.(ty_has_op_type) ot MCCopy⌝ ∗*)
+      ∀ v v', v ◁ᵥ{π} r @ ty -∗
+      T L v' _ (value_t ty.(ty_syn_type)) v val (◁ value_t ty.(ty_syn_type)) (#v) ResultStrong)
+    ⊢ typed_read_end π E L l (◁ ty) (#r) (Owned wl) bmin AllowStrong ot T.
+  Proof.
+    iIntros "(%Hotalg & %Hot & Hs)" (F ???) "#CTX #HE HL Hna".
+    iIntros "_ Hb".
+    iPoseProof (ofty_ltype_acc_owned with "Hb") as "(%ly & %Halg & %Hly & Hsc & Hlb & >(%v & Hl & Hv & Hcl))"; first done.
+    iPoseProof (ty_own_val_has_layout with "Hv") as "%Hlyv"; first done.
+    specialize (ty_op_type_stable Hot) as Halg''.
+    rewrite /use_op_alg' Hotalg in Halg''.
+    assert (ly = ot_layout ot) as ->. { by eapply syn_type_has_layout_inj. }
+    iModIntro. iExists _, _, rt, _, _.
+    iFrame "Hl Hv".
+    iSplitR; first done. iSplitR; first done.
+    iApply (logical_step_wand with "Hcl").
+    iIntros "Hcl %st Hl Hv".
+    iAssert (v ◁ᵥ{π} v @ value_t ty.(ty_syn_type))%I as "Hv'".
+    { rewrite /ty_own_val/=.
+      (*destruct (syn_type_has_layout_op_alg _ _ Halg) as (ot' & Hop & Hot').*)
+      iExists (ot).
+      iR. iSplitR. { iPureIntro. left. done. }
+      iSplitR; last done. iPureIntro. rewrite /has_layout_val . done. }
+    iPoseProof (ty_memcast_compat_copy _ _ _ ot _ st with "Hv'") as "Hv''".
+    { simpl. exists ot. split_and!; first done; last done. by apply is_value_ot_core_refl. }
+    iMod ("Hcl" $! v _ (value_t ty.(ty_syn_type)) (v) with "Hl [//] [] []") as "Hl".
+    { simpl. done. }
+    { iNext. done. }
+    (*iPoseProof (ty_memcast_compat with "Hv") as "Hid"; first done. simpl.*)
+    iModIntro. iExists _, _, (value_t (ty_syn_type ty)), _. iFrame "∗ #".
+    (* strong update *)
+    iExists _, _, _, ResultStrong. iFrame.
+    do 2 iR.
+    iApply "Hs". done.
+  Qed.
+  (* TODO replace the preceding instances with this, once we have fixed:
+      (a) owned_subtype to be able to move stuff into it again reliably, also below structs etc.
+      (b) the model to allow syntype updates as long as the layout stays the same *)
+  (*Global Instance type_read_ofty_move_owned_inst E L {rt} π wl bmin l (ty : type rt) r ot :*)
+    (*TypedReadEnd π E L l (◁ ty)%I (PlaceIn r) (Owned wl) bmin AllowStrong ot | 19 :=*)
+    (*λ T, i2p (type_read_ofty_move_owned E L π T l ty r ot wl bmin).*)
+
+  (* TODO for Untyped, we currently cannot leave a value, because we cannot do syntype updates, but [value_t] relies on the syntype to compute the value update *)
+  Lemma type_read_ofty_move_owned_untyped E L {rt} π (T : typed_read_end_cont_t rt) l (ty : type rt) r ly wl bmin :
+    ( ⌜ty.(ty_has_op_type) (UntypedOp ly) MCCopy⌝ ∗
+      ∀ v v', v ◁ᵥ{π} r @ ty -∗
+      T L v' _ (value_t (UntypedSynType ly)) v val (◁ value_t (UntypedSynType ly)) (#v) ResultStrong) -∗
+      typed_read_end π E L l (◁ ty) (#r) (Owned wl) bmin AllowStrong (UntypedOp ly) T.
+  Proof.
+    iIntros "(%Hot & Hs)" (F ???) "#CTX #HE HL".
+    iIntros "_ Hb".
+  Abort.
+
+  (* Instead we leave uninit *)
+  Lemma type_read_ofty_move_owned_value_untyped E L {rt} π (T : typed_read_end_cont_t rt) l (ty : type rt) r ly wl bmin :
+    (⌜ty.(ty_has_op_type) (UntypedOp ly) MCCopy⌝ ∗
+        ∀ v, T L v _ ty r unit (◁ uninit ty.(ty_syn_type)) (#()) ResultStrong)
+    ⊢ typed_read_end π E L l (◁ ty) (#r) (Owned wl) bmin AllowStrong (UntypedOp ly) T.
+  Proof.
+    iIntros "(%Hot & Hs)" (F ???) "#CTX #HE HL Hna".
+    iIntros "_ Hb".
+    iPoseProof (ofty_ltype_acc_owned with "Hb") as "(%ly' & %Halg & %Hly & Hsc & Hlb & >(%v & Hl & Hv & Hcl))"; first done.
+    iPoseProof (ty_own_val_has_layout with "Hv") as "%Hlyv"; first done.
+    specialize (ty_op_type_stable Hot) as Halg''.
+    assert (ly' = ly) as ->. { by eapply syn_type_has_layout_inj. }
+    iModIntro. iExists _, _, rt, _, _.
+    iFrame "Hl Hv".
+    iSplitR; first done. iSplitR; first done.
+    iApply (logical_step_wand with "Hcl").
+    iIntros "Hcl %st Hl Hv". iMod ("Hcl" $! v _ (uninit ty.(ty_syn_type)) tt with "Hl [//] [] []") as "Hl".
+    { simpl. done. }
+    { iNext. iApply uninit_own_spec. iExists _. iSplitR; first done. done. }
+    iPoseProof (ty_memcast_compat with "Hv") as "Hid"; first done. simpl.
+    iModIntro. iExists _, _,_, _. iFrame.
+    (* strong update *)
+    iExists _, _, _, ResultStrong. iFrame.
+    iSplitR; first done.
+    iR.
+    done.
+  Qed.
+  (*
+  Global Instance type_read_ofty_move_owned_untyped_inst E L {rt} π wl bmin l (ty : type rt) r ly :
+    TypedReadEnd π E L l (◁ ty)%I (PlaceIn r) (Owned wl) bmin AllowStrong (UntypedOp ly) | 20 :=
+    λ T, i2p (type_read_ofty_move_owned_untyped E L π T l ty r ly wl bmin).
+  *)
+
+  (* TODO: this is now problematic. Maybe should have an untyped bit in the syntype after all?
+       Alternative: use syn_type_compat everywhere to allow untyped interaction.
+
+       Use an untyped bit:
+       - then we still have a problem that often we should maybe be talking about a concrete layout instead.
+          In particular when we assemble chunks.
+          For array, we can work around that, since it is "chunkable", but for everything else, that does not really work.
+          Q: do we reallyneed that for anything but arrays?
+          + when we want to have a view on data and change the element type: e.g. in copy_nonoverlapping, would like to have an array of u8.
+            We could in principle also do that for the ArraySynType, but it would be more of a hassle, and we would again end up with a different syntype
+            OTOH is copy_nonoverlapping that much of a concern?
+            In principle, we could also have something that first adapts
+       - making things untyped would be much less of a hassle in the rules.
+
+       Make rules compatible with UntypedSynType everywhere:
+       - what is the intuitive justification for this? Why should we do it?
+         + to my mind, UntypedSynType is just an undesirable artifact -- at least in safe Rust.
+         + for unsafe stuff, the story may be different. We may want to treat stuff just as bytes.
+            - allocation API itself should maybe treat it that way. We should just have some layout there.
+              In our system, we will have a mixed concrete-symbolic layout.
+              Arguably, that should not be a proper syntype, but that's how it is: our types need a syntype, and generally that requirement seems sensible.
+
+       Alternative for this particular issue:
+       - at the place, just don't leave an Untyped, but the right type. We should not loose information there!
+         Then we also do not need a syntype update.
+
+     *)
+
+  (* TODO: consider whether we need special instances for reading/writing.
+     In particular, what if we read with an ot from an UntypedOp-value? Then we should specialize the ot further in the result of the read.
+     - problem currently: the generic ofty instance requires the type to have the same ot
+     - but in case of value_t, we can change the ot!
+   *)
+
+
+
+  (* We also need stratification instances: should we generally move values back in during stratification?
+    - One option: always cancel value_t in stratification.
+        This limits expressivity a bit for specs, because when we really want to have value_t there, we get stuck.
+      => do this for now, it should suffice.
+     - Other option: have a (non-semantic) guidance parameter that gets provided by OpenedLtype.
+       Only if that guidance parameter is not giving us identity do we fold the value_t.
+     - Other option: do not let stratify do this, but rather have subtyping do this before folding.
+
+     TODO: currently not an instance, because we sometimes do not want to do this!
+     Instead, should give stratify some syntactic guidance from OpenedLtype above it.
+   *)
+  Lemma stratify_ltype_ofty_value_owned π E L mu mdu ma {M} (m : M) l st v wl (T : stratify_ltype_cont_t) :
+    find_in_context (FindVal v π) (λ '(existT rt (ty', r')),
+      ⌜ty'.(ty_has_op_type) (use_op_alg' ty'.(ty_syn_type)) MCCopy⌝ ∗
+      ⌜ty'.(ty_syn_type) = st⌝ ∗
+      stratify_ltype π E L mu mdu ma m l (◁ ty') (#r') (Owned wl) T)
+    ⊢ stratify_ltype π E L mu mdu ma m l (◁ value_t st)%I (#v) (Owned wl) T.
+  Proof.
+    iDestruct 1 as ([rt [ty' r']]) "(Hv & %Hot & %Heq & HT)" => /=.
+    iIntros (???) "#CTX #HE HL Hl".
+    iPoseProof (ltype_own_has_layout with "Hl") as "#(%ly & %Hst &_)".
+    iPoseProof (ofty_own_merge_value with "Hv Hl") as "Ha".
+    { subst st. destruct (ty_syn_type ty'); try done.
+      simp_ltypes in Hst. simpl in Hst.
+      specialize (syn_type_has_layout_untyped_inv _ _ Hst) as (-> & _).
+      done. }
+    iMod ("HT" with "[//] [//] CTX HE HL Ha") as "Ha".
+    subst st. eauto.
+  Qed.
+  (* needs to have a higher priority than the ofty_resolve_ghost instance *)
+  (*Global Instance stratify_ltype_unblock_ofty_value_owned_inst π E L mu mdu ma l st v wl :*)
+    (*StratifyLtype π E L mu mdu ma StratifyUnblockOp l (◁ value_t st)%I (PlaceIn v) (Owned wl) | 10:=*)
+    (*λ T, i2p (stratify_ltype_ofty_value_owned π E L mu mdu ma StratifyUnblockOp l st v wl T).*)
+  (* TODO: not an instance right now since we don't always want to stratify this -- esp. not for functions passing values in their interface *)
+
+
+  (* Simplification instance - when introducing a value_t, we simply destruct it *)
+  (* TODO how does this overlap with ghost_drop?
+     TODO can we simplify the is_memcast_val? Otherwise, it seems pretty useless. *)
+  (*
+  Lemma value_simplify π v T ot st p :
+    (⌜is_memcast_val p ot v⌝ -∗ ⌜v `has_layout_val` ot_layout ot⌝ -∗ ⌜syn_type_has_layout st (ot_layout ot)⌝ -∗ T) -∗
+    simplify_hyp (v ◁ᵥ{π} p @ value_t st)%I T.
+  Proof. iIntros "HT (% & % & %)". by iApply "HT". Qed.
+  Global Instance value_simplify_inst π v ot st p :
+    SimplifyHypVal v π (value_t ot st) p (Some 0%N) :=
+    λ T, i2p (value_simplify π v T ot st p).
+   *)
+
+
 
 End rules.
 
